@prefix : <http://www.gsi.upm.es/ontologies/amor/models/mft/ns#> .
@prefix amor: <http://www.gsi.upm.es/ontologies/amor/ns#> .
@prefix dc: <http://purl.org/dc/terms/> .
@prefix mft: <http://www.gsi.upm.es/ontologies/mft/ns#> .
@prefix owl: <http://www.w3.org/2002/07/owl#> .
@prefix rdfs: <http://www.w3.org/2000/01/rdf-schema#> .
@prefix vann: <http://purl.org/vocab/vann/> .
@prefix xsd: <http://www.w3.org/2001/XMLSchema#> .

<http://www.gsi.upm.es/ontologies/amor/models/mft/ns>
  a owl:Ontology ;
  rdfs:label "AMOR-MFT Ontology"@en ;
  owl:versionInfo "1.0.0"^^xsd:string ;
  owl:versionIRI <http://www.gsi.upm.es/ontologies/amor/models/mft/ns/1.0.0> ;
  dc:title "AMOR-MFT Ontology"@en ;
  dc:creator "Sergio Muñoz López"@en ,
    "Álvaro Carrera Barroso"@en ;
  dc:publisher <http://www.gsi.upm.es> ;
  rdfs:comment "AMOR-MFT is an ontology that uses AMOR ontology and MFT SKOS Taxonomy to create required relations to use MFT to define moral annotations."@en ;
  dc:description "AMOR-MFT is an ontology that uses AMOR ontology and MFT SKOS Taxonomy to create required relations to use MFT to define moral annotations."@en ;
  vann:preferredNamespacePrefix "amor-mft" ;
  vann:preferredNamespaceUri "http://www.gsi.upm.es/ontologies/amor/models/mft/ns#" .

:MoralFoundation a owl:Class ;
  rdfs:subClassOf amor:MoralValueCategory ;
  rdfs:label "Moral Foundation"@en ;
  rdfs:comment "A Moral Foundation is a category of moral values, defined by the Moral Foundations Theory, that are used to define the moral values of the annotated content."@en .

:MoralFoundationsTheoryModel a amor:MoralValueModel ;
  rdfs:label "Moral Foundations Theory Model"@en ;
  rdfs:comment "This model uses the 2023 version of the Moral Foundations Theory to define the moral values of the annotated content."@en ;
    amor:hasMoralValueCategory mft:Care ,
        mft:Loyalty ,
        mft:Authority ,
        mft:Purity ,
        mft:Equality ,
        mft:Proportionality ,
        mft:Liberty ,
        mft:Honor ,
        mft:Ownership .

mft:Care a :MoralFoundation .
mft:Fairness a :MoralFoundation .
mft:Loyalty a :MoralFoundation .
mft:Authority  a :MoralFoundation .
mft:Purity  a :MoralFoundation .
mft:Equality  a :MoralFoundation .
mft:Proportionality a :MoralFoundation .
mft:Liberty a :MoralFoundation .
mft:Honor a :MoralFoundation .
mft:Ownership a :MoralFoundation .

:Polarity a owl:Class ;
  rdfs:label "Polarity"@en ;
  rdfs:comment "The polarity is represents the Vice or the Virtue of the MFT Moral Value category."@en .

:hasPolarity
  a owl:ObjectProperty ;
  rdfs:label "has polarity"@en ;
  rdfs:domain amor:MoralValueAnnotation ;
  rdfs:range :Polarity ;
  rdfs:comment "The polarity is represents the Vice or the Virtue of the MFT Moral Value category."@en .

:oppositeOf
  a owl:ObjectProperty ;
  rdfs:label "opposite of"@en ;
  rdfs:domain :Polarity ;
  rdfs:range :Polarity ;
  rdfs:comment "The opposite of a polarity is the opposite polarity."@en .

mft:Virtue a :Polarity ;
  :oppositeOf mft:Vice ;
  rdfs:label "Vice"@en ,
    "Vicio"@es .

mft:Vice a :Polarity ;
  :oppositeOf mft:Virtue ;
  rdfs:label "Virtue"@en ,
    "Virtud"@es .

:hasPolarityIntensity
  a owl:DatatypeProperty ;
  rdfs:label "has polarity intensity"@en ;
  rdfs:domain amor:MoralValueAnnotation ;
  rdfs:range xsd:float ;
  rdfs:comment "The polarity of a moral value annotation represents the intensity of the moral value in the analyzed textual source, ranging from -1.0 (for vice) to 1.0 (for virtue)."@en .