@prefix : <http://www.gsi.upm.es/ontologies/amor/experiments/ns#> .
@prefix dc: <http://purl.org/dc/terms/> .
@prefix foaf: <http://xmlns.com/foaf/0.1/> .
@prefix oa: <http://www.w3.org/ns/oa#> .
@prefix oro: <http://kb.openrobots.org#> .
@prefix owl: <http://www.w3.org/2002/07/owl#> .
@prefix prov: <http://www.w3.org/ns/prov#> .
@prefix rdfs: <http://www.w3.org/2000/01/rdf-schema#> .
@prefix schema: <http://schema.org/> .
@prefix segb: <http://www.gsi.upm.es/ontologies/segb/ns#> .
@prefix vann: <http://purl.org/vocab/vann/> .
@prefix xml: <http://www.w3.org/XML/1998/namespace/> .
@prefix xsd: <http://www.w3.org/2001/XMLSchema#> .

<http://www.gsi.upm.es/ontologies/amor/experiments/ns>
    a owl:Ontology ;
    rdfs:label "AMOR Experiments Ontology"@en ;
    owl:versionInfo "1.0.0"^^xsd:string ;
    owl:versionIRI <http://www.gsi.upm.es/ontologies/amor/experiments/ns/1.0.0> ;
    dc:title "AMOR Experiments Ontology"@en ;
    dc:creator "√Ålvaro Carrera Barroso"@en ;
    dc:publisher <http://www.gsi.upm.es> ;
    rdfs:comment "AMOR Experiments is an ontology designed for representing experiments and evaluations in the AMOR project."@en ;
    dc:description "AMOR Experiments is an ontology designed for representing experiments and evaluations in the AMOR project."@en ;
    vann:preferredNamespacePrefix "amor-exp" ;
    vann:preferredNamespaceUri "http://www.gsi.upm.es/ontologies/amor/experiments/ns#" .

# Parameter 1: Experiment identifier
:Experiment
    a owl:Class ;
    rdfs:subClassOf prov:Activity ;
    rdfs:label "Experiment"@en ;
    rdfs:comment "Represents an experiment in the AMOR project."@en .

:isRelatedWithExperiment
    a owl:ObjectProperty ;
    rdfs:subPropertyOf prov:wasAssociatedWith ;
    rdfs:domain segb:LoggedActivity ;
    rdfs:range :Experiment ;
    rdfs:label "is related with experiment"@en ;
    rdfs:comment "Relates an activity logged in the AMOR-SEGB with the experiment in progress."@en .

:ExperimentationSubject
    a owl:Class ;
    rdfs:subClassOf prov:Agent ;
    rdfs:label "Experimentation Subject"@en ;
    rdfs:comment "Represents a subject of an experiment in the AMOR project."@en .

:ExperimentExecutor
    a owl:Class ;
    rdfs:subClassOf prov:Agent ;
    rdfs:label "Experiment Executor"@en ;
    rdfs:comment "Represents an executor of an experiment in the AMOR project."@en .

:ExperimentRequester
    a owl:Class ;
    rdfs:subClassOf prov:Agent ;
    rdfs:label "Experiment Requester"@en ;
    rdfs:comment "Represents a requester of an experiment in the AMOR project."@en .

:hasExperimentationSubject
    a owl:ObjectProperty ;
    rdfs:domain :Experiment ;
    rdfs:range :ExperimentionSubject ;
    rdfs:label "has experimentation subject"@en ;
    rdfs:comment "Relates an experiment with its subject."@en .

:hasExecutor
    a owl:ObjectProperty ;
    rdfs:domain :Experiment ;
    rdfs:range :ExperimentExecutor ;
    rdfs:label "has experiment executor"@en ;
    rdfs:comment "Relates an experiment with its executor."@en .

:hasRequester
    a owl:ObjectProperty ;
    rdfs:domain :Experiment ;
    rdfs:range :ExperimentRequester ;
    rdfs:label "has experiment requester"@en ;
    rdfs:comment "Relates an experiment with its requester, i.e. the person who requests the execution of the experiment."@en .

:ExperimentParameter
    a owl:Class ;
    rdfs:subClassOf prov:Entity ;
    rdfs:label "Experiment Parameter"@en ;
    rdfs:comment "Represents a parameter of an experiment in the AMOR project."@en .

:hasParameter
    a owl:ObjectProperty ;
    rdfs:domain :Experiment ;
    rdfs:range owl:Thing ;
    rdfs:label "has parameter"@en ;
    rdfs:comment "Relates an experiment with its parameters."@en .

# Types of experiments defined for the AMOR project.

:DigitalNewspaperExperiment 
    a owl:Class ;
    rdfs:subClassOf :Experiment ;
    rdfs:label "Digital Newspaper Experiment"@en ;
    rdfs:comment "Represents an experiment with a digital newspaper in the AMOR project."@en .

:MoralValuesExperiment
    a owl:Class ;
    rdfs:subClassOf :DigitalNewspaperExperiment ;
    rdfs:label "Moral Values Experiment"@en ;
    rdfs:comment "Represents an experiment with moral values in the AMOR project."@en .

:MoralFrameExperiment
    a owl:Class ;
    rdfs:subClassOf :DigitalNewspaperExperiment ;
    rdfs:label "Moral Frame Experiment"@en ;
    rdfs:comment "Represents an experiment with a moral frame in the AMOR project."@en .

:SearchEngineBiasExperiment
    a owl:Class ;
    rdfs:subClassOf :DigitalNewspaperExperiment ;
    rdfs:label "Search Engine Bias Experiment"@en ;
    rdfs:comment "Represents an experiment with a search engine bias in the AMOR project."@en .

:ClickBaitExperiment
    a owl:Class ;
    rdfs:subClassOf :DigitalNewspaperExperiment ;
    rdfs:label "Click Bait Experiment"@en ;
    rdfs:comment "Represents an experiment with click bait in the AMOR project."@en .

:FakeNewsAwarenessExperiment
    a owl:Class ;
    rdfs:subClassOf :DigitalNewspaperExperiment ;
    rdfs:label "Fake News Awareness Experiment"@en ;
    rdfs:comment "Represents an experiment with fake news awareness in the AMOR project."@en .

:SocialNetworkExperiment
    a owl:Class ;
    rdfs:subClassOf :Experiment ;
    rdfs:label "Social Network Experiment"@en ;
    rdfs:comment "Represents an experiment with a social network in the AMOR project."@en .

:GeographicalVisualizationExperiment
    a owl:Class ;
    rdfs:subClassOf :Experiment ;
    rdfs:label "Geographical Visualization Experiment"@en ;
    rdfs:comment "Represents an experiment with geographical visualization in the AMOR project."@en .

# Types of parameters defined for the AMOR project.

# Parameter 2: Content used in the experiment
:usesDataset
    a owl:ObjectProperty ;
    rdfs:subPropertyOf :hasParameter ;
    rdfs:domain :DigitalNewspaperExperiment ;
    rdfs:range :NewsDataset ;
    rdfs:label "has dataset"@en ;
    rdfs:comment "Relates a news content dataset parameter with its dataset."@en .

:NewsDataset a owl:Class ;
    rdfs:subClassOf schema:Dataset ;
    rdfs:subClassOf :ExperimentParameter ;
    rdfs:label "News Dataset"@en ;
    rdfs:comment "Represents a dataset of news content."@en .

:hasNews
    a owl:ObjectProperty ;
    rdfs:subPropertyOf schema:hasPart ;
    rdfs:domain :NewsDataset ;
    rdfs:range schema:NewsArticle ;
    rdfs:label "has main entity"@en ;
    rdfs:comment "Relates a news dataset with its main entity."@en .

# Parameter 3: Recommended content (news) in the experiment
## Replaced with oa:hasBody in :Recommendation nodes
#:hasRecommendation
#    a owl:ObjectProperty ;
#    rdfs:subPropertyOf schema:subjectOf ;
#    rdfs:domain schema:NewsArticle ;
#    rdfs:range :Recommendation ;
#    rdfs:label "has recommendation"@en ;
#    rdfs:comment "Represents a recommendation that recommends a news based on a specific criterion."@en .

:hasRecommendationCriterion
    a owl:ObjectProperty ;
    rdfs:subPropertyOf schema:category ;
    rdfs:domain :Recommendation ;
    rdfs:range :RecommendationCriterion ;
    rdfs:label "has recommendation criterion"@en ;
    rdfs:comment "Relates a recommendation with its recommendation criterion."@en .

## Replaced with oa:hasTarget
#:hasRecommendedNews a owl:ObjectProperty ;
#    rdfs:domain :Recommendation ;
#    rdfs:range schema:NewsArticle ;
#    rdfs:label "has recommended news"@en ;
#    rdfs:comment "Relates a recommendation with the news article recommended."@en .

:hasRecommendationScore a owl:DatatypeProperty ;
    rdfs:domain :Recommendation ;
    rdfs:range xsd:float ;
    rdfs:label "has recommendation score"@en ;
    rdfs:comment "Relates a recommendation with the score of the recommendation."@en .

:Recommendation
        a owl:Class;
    rdfs:subClassOf oa:Recommendation ;
    rdfs:label "Recommendation"@en ;
    rdfs:comment "Represents a recommendation for a piee of content."@en .

:RecommendationStrategyParameter
        a owl:Class;
    rdfs:subClassOf :ExperimentParameter ;
    rdfs:label "Recommendation Strategy Parameter"@en ;
    rdfs:comment "Represents the strategy used to filter recommendations for an item in an experiment in the AMOR project."@en .

:hasRecommendationStrategy
    a owl:ObjectProperty ;
    rdfs:subPropertyOf :hasParameterValue ;
    rdfs:domain :RecommendationStrategyParameter ;
    rdfs:range :RecommendationCriterion ;
    rdfs:label "has recommendation strategy"@en ;
    rdfs:comment "Relates a recommendation strategy parameter with its recommentation strategy."@en .

:RecommendationCriterion
    a owl:Class ;
    rdfs:label "Recommendation Criterion"@en ;
    rdfs:comment "Represents a criterion used to filter recommendations in an experiment in the AMOR project."@en .

:MoralSimilarity
    a owl:NamedIndividual, :RecommendationCriterion ;
    rdfs:label "Similar Moral Recommendation Strategy"@en ;
    rdfs:comment "Recommends elements with a similar moral value"@en .

:MoralDissimilarity
    a owl:NamedIndividual, :RecommendationCriterion ;
    rdfs:label "Opposite Moral Recommendation Strategy"@en ;
    rdfs:comment "Recommends elements with an opposite moral value"@en .

:EmotionSimilarity
    a owl:NamedIndividual, :RecommendationCriterion ;
    rdfs:label "Similar Emotion Recommendation Strategy"@en ;
    rdfs:comment "Recommends elements with a similar emotion value"@en .

:EmotionDissimilarity
    a owl:NamedIndividual, :RecommendationCriterion ;
    rdfs:label "Opposite Emotion Recommendation Strategy"@en ;
    rdfs:comment "Recommends elements with an opposite emotion value"@en .

:SentimentSimilarity
    a owl:NamedIndividual, :RecommendationCriterion ;
    rdfs:label "Similar Sentiment Recommendation Strategy"@en ;
    rdfs:comment "Recommends elements with a similar sentiment value"@en .

:SentimentDisimilarity
    a owl:NamedIndividual, :RecommendationCriterion ;
    rdfs:label "Opposite Sentiment Recommendation Strategy"@en ;
    rdfs:comment "Recommends elements with an opposite sentiment value"@en .

:EntitySimilarity
    a owl:NamedIndividual, :RecommendationCriterion ;
    rdfs:label "Similar Entities Recommendation Strategy"@en ;
    rdfs:comment "Recommends elements with a similar named entities"@en .

# Parameter 4: Visualization strategy used in the experiment
:hasVisualizationStrategy
    a owl:ObjectProperty ;
    rdfs:subPropertyOf :hasParameter ;
    rdfs:domain :Experiment ;
    rdfs:range :VisualizationStrategy ;
    rdfs:label "has visualization strategy"@en ;
    rdfs:comment "Relates an experiment with its visualization strategy."@en .

:VisualizationStrategy
    a owl:Class ;
    rdfs:label "Visualization Strategy"@en ;
    rdfs:comment "Represents a strategy used to visualize the results of an experiment in the AMOR project."@en .

:MoralValueVisualizationStrategy
    a owl:NamedIndividual, :VisualizationStrategy ;
    rdfs:label "Moral Value Visualization Strategy"@en ;
    rdfs:comment "Represents the strategy used to visualize the moral values of the results of an experiment in the AMOR project."@en .

:AffectiveValueVisualizationStrategy
    a owl:NamedIndividual, :VisualizationStrategy ;
    rdfs:label "Affective Value Visualization Strategy"@en ;
    rdfs:comment "Represents the strategy used to visualize the affective values of the results of an experiment in the AMOR project."@en .

:ClickBaitVisualizationStrategy
    a owl:NamedIndividual, :VisualizationStrategy ;
    rdfs:label "Click Bait Visualization Strategy"@en ;
    rdfs:comment "Represents the strategy used to visualize the click bait values of the results of an experiment in the AMOR project."@en .

:FakeNewsVisualizationStrategy
    a owl:NamedIndividual, :VisualizationStrategy ;
    rdfs:label "Fake News Visualization Strategy"@en ;
    rdfs:comment "Represents the strategy used to visualize the fake news values of the results of an experiment in the AMOR project."@en .

# Parameter 5: Information about the experimentation subject (user) in the experiment
:hasAgeBracket
    a owl:DatatypeProperty ;
    rdfs:domain :ExperimentionSubject ;
    rdfs:range xsd:string ;
    rdfs:label "has age bracket"@en ;
    rdfs:comment "Relates an experimentation subject with its age bracket."@en .

:hasPoliticalOrientation
    a owl:DatatypeProperty ;
    rdfs:domain :ExperimentionSubject ;
    rdfs:range xsd:string ;
    rdfs:label "has political orientation"@en ;
    rdfs:comment "Relates an experimentation subject with its political orientation."@en .

:hasStressLevel
    a owl:DatatypeProperty ;
    rdfs:domain :ExperimentionSubject ;
    rdfs:range xsd:float ;
    rdfs:label "has stress level"@en ;
    rdfs:comment "Relates an experimentation subject with its stress level (between 0.0 to 1.0)."@en .

:hasAccesibilityCategory
    a owl:DatatypeProperty ;
    rdfs:domain :ExperimentionSubject ;
    rdfs:range xsd:string ;
    rdfs:label "has accesibility category"@en ;
    rdfs:comment "Relates an experimentation subject with its accesibility category."@en .

:hasEducationalLevel
    a owl:DatatypeProperty ;
    rdfs:domain :ExperimentionSubject ;
    rdfs:range xsd:string ;
    rdfs:label "has educational level"@en ;
    rdfs:comment "Relates an experimentation subject with its educational level."@en .

:hasPreferredContent
    a owl:ObjectProperty ;
    rdfs:domain :ExperimentionSubject ;
    rdfs:range schema:CreativeWork ;
    rdfs:label "has preferred content"@en ;
    rdfs:comment "Relates an experimentation subject with its preferred content."@en .

:hasPreferredTopic
    a owl:DatatypeProperty ;
    rdfs:domain :ExperimentionSubject ;
    rdfs:range xsd:string ;
    rdfs:label "has preferred topic"@en ;
    rdfs:comment "Relates an experimentation subject with its preferred topic."@en .

:hasPreferredEntity
    a owl:DatatypeProperty ;
    rdfs:domain :ExperimentionSubject ;
    rdfs:range prov:Entity ;
    rdfs:label "has preferred entities"@en ;
    rdfs:comment "Relates an experimentation subject with its preferred entities."@en .

:hasNumberOfFollowers
    a owl:DatatypeProperty ;
    rdfs:domain :ExperimentionSubject ;
    rdfs:range xsd:integer ;
    rdfs:label "has number of followers"@en ;
    rdfs:comment "Relates an experimentation subject with the number of followers."@en .

:hasAverageSocialNetworkActivityPerMonth
    a owl:DatatypeProperty ;
    rdfs:domain :ExperimentionSubject ;
    rdfs:range xsd:integer ;
    rdfs:label "has average social network activity per month"@en ;
    rdfs:comment "Relates an experimentation subject with the average social network activity per month."@en .

# Parameter 6: Language used in the experiment
:usesLanguage
    a owl:DatatypeProperty ;
    rdfs:subPropertyOf :hasParameter ;
    rdfs:domain :Experiment ;
    rdfs:range xml:lang ;
    rdfs:label "uses language"@en ;
    rdfs:comment "Relates a digital newspaper experiment with the language used in the experiment."@en .

# Parameter 7: Robot/Hollographic Character used in the experiment

:usesAvatar
    a owl:ObjectProperty ;
    rdfs:subPropertyOf :hasParameter ;
    rdfs:domain :Experiment ;
    rdfs:range :Avatar ;
    rdfs:label "uses avatar"@en ;
    rdfs:comment "Relates an experiment with the avatar used."@en .

:Avatar
    a owl:Class ;
    rdfs:subClassOf foaf:Agent ;
    rdfs:label "Avatar"@en ;
    rdfs:comment "Represents an avatar used in an experiment in the AMOR project."@en .

:hasCategory
    a owl:DatatypeProperty ;
    rdfs:domain :Avatar ;
    rdfs:range xsd:string ;
    rdfs:label "has category"@en ;
    rdfs:comment "Relates a character with its category."@en .

:hasAppearance
    a owl:DatatypeProperty ;
    rdfs:domain :Avatar ;
    rdfs:range xsd:string ;
    rdfs:label "has appearance"@en ;
    rdfs:comment "Relates a character with its appearance."@en .

:hasPersonality
    a owl:DatatypeProperty ;
    rdfs:domain :Avatar ;
    rdfs:range xsd:string ;
    rdfs:label "has personality"@en ;
    rdfs:comment "Relates a character with its personality."@en .

:hasVoice
    a owl:DatatypeProperty ;
    rdfs:domain :Avatar ;
    rdfs:range xsd:string ;
    rdfs:label "has voice"@en ;
    rdfs:comment "Relates a character with its voice."@en .

:hasLanguageComplexityLevel
    a owl:DatatypeProperty ;
    rdfs:domain :Avatar ;
    rdfs:range xsd:string ;
    rdfs:label "has language complexity level"@en ;
    rdfs:comment "Relates a character with its language complexity level."@en .

# Parameter 8, 9 & 10: Expresivity levels used in the experiment
:ExpresivityCategory
    a owl:Class ;
    rdfs:label "Expresivity Category"@en ;
    rdfs:comment "Represents the expresivity category of a character in an experiment in the AMOR project."@en .

:NoExpresivity
    a owl:NamedIndividual, :ExpresivityCategory ;
    rdfs:label "No Expresivity"@en ;
    rdfs:comment "Represents the absence of expresivity in a character."@en .

:EmotiveExpresivity
    a owl:NamedIndividual, :ExpresivityCategory ;
    rdfs:label "Emotive Expresivity"@en ;
    rdfs:comment "Represents the emotive expresivity of a character."@en .

:EmphaticExpresivity
    a owl:NamedIndividual, :ExpresivityCategory ;
    rdfs:label "Emphatic Expresivity"@en ;
    rdfs:comment "Represents the emphatic expresivity of a character."@en .

:ExaggeratedExpresivity
    a owl:NamedIndividual, :ExpresivityCategory ;
    rdfs:label "Exaggerated Expresivity"@en ;
    rdfs:comment "Represents the exaggerated expresivity of a character."@en .

:hasFacialExpresivity
    a owl:ObjectProperty ;
    rdfs:domain :Avatar ;
    rdfs:range :ExpresivityCategory ;
    rdfs:label "has facial expresivity"@en ;
    rdfs:comment "Relates a character with its facial expresivity."@en .

:hasGesturalExpresivity
    a owl:ObjectProperty ;
    rdfs:domain :Avatar ;
    rdfs:range :ExpresivityCategory ;
    rdfs:label "has gestural expresivity"@en ;
    rdfs:comment "Relates a character with its gestural expresivity."@en .

:hasVocalExpresivity
    a owl:ObjectProperty ;
    rdfs:domain :Avatar ;
    rdfs:range :ExpresivityCategory ;
    rdfs:label "has vocal expresivity"@en ;
    rdfs:comment "Relates a character with its vocal expresivity."@en .

# Parameter 11: Content Adaptation Strategy used in the experiment
:ContentAdaptationStrategy
    a owl:Class ;
    rdfs:label "Content Adaptation Strategy"@en ;
    rdfs:comment "Represents a strategy used to adapt the content in an experiment in the AMOR project."@en .

:hasContentAdaptationStrategy
    a owl:ObjectProperty ;
    rdfs:subPropertyOf :hasParameter ;
    rdfs:domain :Experiment ;
    rdfs:range :ContentAdaptationStrategy ;
    rdfs:label "has content adaptation strategy"@en ;
    rdfs:comment "Relates an experiment with the content adaptation strategy used."@en .

:NoAdaptationStrategy
    a owl:NamedIndividual, :ContentAdaptationStrategy ;
    rdfs:label "No Adaptation Strategy"@en ;
    rdfs:comment "Represents the absence of content adaptation strategy."@en .

:MoralAdaptationStrategy
    a owl:NamedIndividual, :ContentAdaptationStrategy ;
    rdfs:label "Moral Adaptation Strategy"@en ;
    rdfs:comment "Represents the moral adaptation strategy."@en .

:AfectiveAdaptationStrategy
    a owl:NamedIndividual, :ContentAdaptationStrategy ;
    rdfs:label "Affective Adaptation Strategy"@en ;
    rdfs:comment "Represents the affective adaptation strategy."@en .

# Parameter 12: Robot's physical movement used in the experiment
:hasPhysicalMovement
    a owl:DatatypeProperty ;
    rdfs:subPropertyOf :hasParameter ;
    rdfs:domain :Experiment ;
    rdfs:range xsd:string ;
    rdfs:label "has physical movement"@en ;
    rdfs:comment "Relates an experiment with the physical movement used."@en .

# Parameter 13: Background scenario used in the experiment
:hasBackgroundScenario
    a owl:DatatypeProperty ;
    rdfs:subPropertyOf :hasParameter ;
    rdfs:domain :Experiment ;
    rdfs:range xsd:string ;
    rdfs:label "has background scenario"@en ;
    rdfs:comment "Relates an experiment with the background scenario used."@en .

# Parameter 14: Aggregated data used in the experiment
:usesAggregatedData
    a owl:DatatypeProperty ;
    rdfs:subPropertyOf :hasParameter ;
    rdfs:domain :Experiment ;
    rdfs:range xsd:string ;
    rdfs:label "uses aggregated data"@en ;
    rdfs:comment "Relates an experiment with the aggregated data used."@en .

# Parameter 15: Background music used in the experiment
:hasBackgroundMusic
    a owl:DatatypeProperty ;
    rdfs:domain :Experiment ;
    rdfs:range xsd:string ;
    rdfs:label "has background music"@en ;
    rdfs:comment "Relates an experiment with the background music used."@en .

# Parameter 16: LLM used in the experiment
:LLMConfiguration
    a owl:Class ;
    rdfs:label "LLM Configuration"@en ;
    rdfs:comment "Represents the configuration of the LLM used in an experiment in the AMOR project."@en .

:hasLLMConfiguration
    a owl:ObjectProperty ;
    rdfs:subPropertyOf :hasParameter ;
    rdfs:domain :Experiment ;
    rdfs:range :LLMConfiguration ;
    rdfs:label "has LLM configuration"@en ;
    rdfs:comment "Relates an experiment with the LLM configuration used."@en .

:usesLLMService
    a owl:DatatypeProperty ;
    rdfs:domain :LLMConfiguration ;
    rdfs:range xsd:string ;
    rdfs:label "uses LLM service"@en ;
    rdfs:comment "Relates an LLM configuration with the LLM service used."@en .

:usesLLMEndPoint
    a owl:DatatypeProperty ;
    rdfs:domain :LLMConfiguration ;
    rdfs:range xsd:string ;
    rdfs:label "uses LLM end point"@en ;
    rdfs:comment "Relates an LLM configuration with the LLM end point used."@en .

:hasLLMToken
    a owl:DatatypeProperty ;
    rdfs:domain :LLMConfiguration ;
    rdfs:range xsd:string ;
    rdfs:label "has LLM token"@en ;
    rdfs:comment "Relates an LLM configuration with the LLM token used."@en .

:usesLLMModel
    a owl:DatatypeProperty ;
    rdfs:domain :LLMConfiguration ;
    rdfs:range xsd:string ;
    rdfs:label "uses LLM model"@en ;
    rdfs:comment "Relates an LLM configuration with the LLM model used."@en .

:usesPrompt
    a owl:DatatypeProperty ;
    rdfs:domain :LLMConfiguration ;
    rdfs:range xsd:string ;
    rdfs:label "uses prompt"@en ;
    rdfs:comment "Relates an LLM configuration with the prompt used."@en .

# Parameter 17, 18 & 19: Semantic cooperation strategy used in the experiment
:usesSemanticCooperationConfiguration
    a owl:ObjectProperty ;
    rdfs:subPropertyOf :hasParameter ;
    rdfs:domain :Experiment ;
    rdfs:range :SemanticCooperationConfiguration ;
    rdfs:label "uses semantic cooperation strategy"@en ;
    rdfs:comment "Relates an experiment with the semantic cooperation strategy used."@en .

:SemanticCooperationConfiguration
    a owl:Class ;
    rdfs:label "Semantic Cooperation Configuration"@en ;
    rdfs:comment "Represents the configuration of the semantic cooperation used in an experiment in the AMOR project."@en . 

:usesSemanticCooperationStrategy
    a owl:ObjectProperty ;
    rdfs:subPropertyOf :hasParameter ;
    rdfs:domain :SemanticCooperationConfiguration ;
    rdfs:range :SemanticCooperationStrategy ;
    rdfs:label "uses semantic cooperation strategy"@en ;
    rdfs:comment "Relates an experiment with the semantic cooperation strategy used."@en .

:SemanticCooperationStrategy
    a owl:Class ;
    rdfs:label "Semantic Cooperation Strategy"@en ;
    rdfs:comment "Represents the strategy used to cooperate with the semantic web in an experiment in the AMOR project."@en .

:NoSemanticCooperation
    a owl:NamedIndividual, :SemanticCooperationStrategy ;
    rdfs:label "No Semantic Cooperation"@en ;
    rdfs:comment "Represents the absence of semantic cooperation in an experiment."@en .

:FullSemanticCooperation
    a owl:NamedIndividual, :SemanticCooperationStrategy ;
    rdfs:label "Full Semantic Cooperation"@en ;
    rdfs:comment "Represents the full semantic cooperation in an experiment."@en .

:LocalSemanticCooperation
    a owl:NamedIndividual, :SemanticCooperationStrategy ;
    rdfs:label "Local Semantic Cooperation"@en ;
    rdfs:comment "Represents the local semantic cooperation in an experiment."@en .

:CloudSemanticCooperation
    a owl:NamedIndividual, :SemanticCooperationStrategy ;
    rdfs:label "Cloud Semantic Cooperation"@en ;
    rdfs:comment "Represents the cloud semantic cooperation in an experiment."@en .

# Parameter 18: SPARQL query used in the experiment
:usesSPARQLQuery
    a owl:DatatypeProperty ;
    rdfs:domain :SemanticCooperationConfiguration ;
    rdfs:range xsd:string ;
    rdfs:label "uses SPARQL query"@en ;
    rdfs:comment "Relates a semantic cooperation strategy with the SPARQL query used."@en .

# Parameter 19: Cloud graph query used in the experiment
:usesCloudGraphQuery
    a owl:DatatypeProperty ;
    rdfs:domain :SemanticCooperationConfiguration ;
    rdfs:range xsd:string ;
    rdfs:label "uses cloud graph query"@en ;
    rdfs:comment "Relates a semantic cooperation strategy with the cloud graph query used."@en .

# Parameter 20: Emotion recognition cooperation strategy used in the experiment
:usesEmotionRecognitionCooperationStrategy
    a owl:ObjectProperty ;
    rdfs:subPropertyOf :hasParameter ;
    rdfs:domain :Experiment ;
    rdfs:range :EmotionRecognitionCooperationStrategy ;
    rdfs:label "uses emotion recognition cooperation configuration"@en ;
    rdfs:comment "Relates an experiment with the emotion recognition cooperation configuration used."@en .

:EmotionRecognitionCooperationStrategy
    a owl:Class ;
    rdfs:label "Emotion Recognition Cooperation Strategy"@en ;
    rdfs:comment "Represents the strategy used to cooperate with the emotion recognition in an experiment in the AMOR project."@en .

:NoCooperationEmotionRecognition
    a owl:NamedIndividual, :EmotionRecognitionCooperationStrategy ;
    rdfs:label "No Cooperation Emotion Recognition"@en ;
    rdfs:comment "Represents the absence of cooperation in emotion recognition in an experiment."@en .

:FullCooperationEmotionRecognition
    a owl:NamedIndividual, :EmotionRecognitionCooperationStrategy ;
    rdfs:label "Full Cooperation Emotion Recognition"@en ;
    rdfs:comment "Represents the full cooperation in emotion recognition in an experiment."@en .

:LocalEmotionRecognition
    a owl:NamedIndividual, :EmotionRecognitionCooperationStrategy ;
    rdfs:label "Local Cooperation Emotion Recognition"@en ;
    rdfs:comment "Represents the local cooperation in emotion recognition in an experiment."@en .

:CloudEmotionRecognition
    a owl:NamedIndividual, :EmotionRecognitionCooperationStrategy ;
    rdfs:label "Cloud Cooperation Emotion Recognition"@en ;
    rdfs:comment "Represents the cloud cooperation in emotion recognition in an experiment."@en .

# Parameter 21: Robot cooperation strategy used in the experiment
:usesRobotCooperationConfiguration
    a owl:ObjectProperty ;
    rdfs:subPropertyOf :hasParameter ;
    rdfs:domain :Experiment ;
    rdfs:range :RobotCooperationConfiguration ;
    rdfs:label "uses robot cooperation configuration"@en ;
    rdfs:comment "Relates an experiment with the robot cooperation configuration used."@en .

:usesRobotCooperationStrategy
    a owl:ObjectProperty ;
    rdfs:subPropertyOf :hasParameter ;
    rdfs:domain :RobotCooperationConfiguration ;
    rdfs:range :RobotCooperationStrategy ;
    rdfs:label "uses robot cooperation strategy"@en ;
    rdfs:comment "Relates a robot cooperation configuration with the robot cooperation strategy used."@en .

:RobotCooperationStrategy
    a owl:Class ;
    rdfs:label "Robot Cooperation Strategy"@en ;
    rdfs:comment "Represents the strategy used to cooperate with the robot in an experiment in the AMOR project."@en .

:NoCooperationRobot
    a owl:NamedIndividual, :RobotCooperationStrategy ;
    rdfs:label "No Cooperation Robot"@en ;
    rdfs:comment "Represents the absence of cooperation in robot in an experiment."@en .

:CooperationRobots
    a owl:NamedIndividual, :RobotCooperationStrategy ;
    rdfs:label "Cognitive Cooperation Robot"@en ;
    rdfs:comment "Represents the cognitive cooperation in robot in an experiment."@en .

:CompetitiveRobots
    a owl:NamedIndividual, :RobotCooperationStrategy ;
    rdfs:label "Competitive Cooperation Robot"@en ;
    rdfs:comment "Represents the competitive cooperation in robot in an experiment."@en .

:hasRobotRole
    a owl:DatatypeProperty ;
    rdfs:domain :RobotCooperationConfiguration ;
    rdfs:range :RobotRole ;
    rdfs:label "has robot role"@en ;
    rdfs:comment "Relates a robot cooperation strategy with the robot role."@en .

:RobotRole
    a owl:Class ;
    rdfs:label "Robot Role"@en ;
    rdfs:comment "Represents the role of a robot in an experiment in the AMOR project."@en .

:hasRobotActor
    a owl:DatatypeProperty ;
    rdfs:domain :RobotRole ;
    rdfs:range oro:Robot ;
    rdfs:label "has robot actor"@en ;
    rdfs:comment "Relates a robot role with the robot actor."@en .

:hasRoleType
    a owl:DatatypeProperty ;
    rdfs:domain :RobotRole ;
    rdfs:range xsd:string ;
    rdfs:label "has robot role type"@en ;
    rdfs:comment "Relates a robot role with the robot role type."@en .

# Parameter 22: Robot cooperation strategy used in the experiment
:ExperimentEvaluation
    a owl:Class ;
    rdfs:subClassOf prov:Entity ;
    rdfs:label "Experiment Evaluation"@en ;
    rdfs:comment "Represents an evaluation of an experiment in the AMOR project."@en .

:hasExperimentEvaluation
    a owl:ObjectProperty ;
    rdfs:subPropertyOf :hasParameter ;
    rdfs:domain :Experiment ;
    rdfs:range :ExperimentEvaluation ;
    rdfs:label "has experiment evaluation"@en ;
    rdfs:comment "Relates an experiment with its evaluation."@en .

:hasInitialQuestion
    a owl:ObjectProperty ;
    rdfs:domain :ExperimentEvaluation ;
    rdfs:range schema:Question ;
    rdfs:label "has initial question"@en ;
    rdfs:comment "Relates an experiment evaluation with the initial questionnaire."@en .

:hasIntermediateQuestion
    a owl:ObjectProperty ;
    rdfs:domain :ExperimentEvaluation ;
    rdfs:range schema:Question ;
    rdfs:label "has intermediate question"@en ;
    rdfs:comment "Relates an experiment evaluation with the intermediate questionnaire."@en .

:hasFinalQuestion
    a owl:ObjectProperty ;
    rdfs:domain :ExperimentEvaluation ;
    rdfs:range schema:Question ;
    rdfs:label "has final question"@en ;
    rdfs:comment "Relates an experiment evaluation with the final questionnaire."@en .

:LikertQuestion
    a owl:Class ;
    rdfs:subClassOf schema:Question ,
        [
        a owl:Restriction ;
        owl:onProperty schema:suggestedAnswer ;
        owl:allValuesFrom [
            a owl:Class ;
            owl:unionOf (
                [
                    a owl:Restriction ;
                    owl:onProperty schema:suggestedAnswer ;
                    owl:allValuesFrom [
                        a owl:Class ;
                        owl:oneOf (
                            [
                                a schema:Answer ;
                                schema:text "Strongly Disagree"^^xsd:string
                            ]
                            [
                                a schema:Answer ;
                                schema:text "Disagree"^^xsd:string
                            ]
                            [
                                a schema:Answer ;
                                schema:text "Neutral"^^xsd:string
                            ]
                            [
                                a schema:Answer ;
                                schema:text "Agree"^^xsd:string
                            ]
                            [
                                a schema:Answer ;
                                schema:text "Strongly Agree"^^xsd:string
                            ]
                        )
                    ]
                ]
                [
                    a owl:Restriction ;
                    owl:onProperty schema:suggestedAnswer ;
                    owl:allValuesFrom [
                        a owl:Class ;
                        owl:oneOf (
                            [
                                a schema:Answer ;
                                schema:text "1"^^xsd:string
                            ]
                            [
                                a schema:Answer ;
                                schema:text "2"^^xsd:string
                            ]
                            [
                                a schema:Answer ;
                                schema:text "3"^^xsd:string
                            ]
                            [
                                a schema:Answer ;
                                schema:text "4"^^xsd:string
                            ]
                            [
                                a schema:Answer ;
                                schema:text "5"^^xsd:string
                            ]
                        )
                    ]
                ]
            )
        ]
        ] ;
    rdfs:label "Likert Question"@en ;
    rdfs:comment "Represents a Likert question."@en .
