@prefix : <http://www.gsi.upm.es/ontologies/amor/experiments/ns#> .
@prefix owl: <http://www.w3.org/2002/07/owl#> .
@prefix rdf: <http://www.w3.org/1999/02/22-rdf-syntax-ns#> .
@prefix xml: <http://www.w3.org/XML/1998/namespace> .
@prefix xsd: <http://www.w3.org/2001/XMLSchema#> .
@prefix rdfs: <http://www.w3.org/2000/01/rdf-schema#> .
@base <http://www.gsi.upm.es/ontologies/amor/experiments/ns#> .

<http://www.gsi.upm.es/ontologies/amor/experiments/ns> rdf:type owl:Ontology ;
                                                        owl:versionIRI <http://www.gsi.upm.es/ontologies/amor/experiments/ns/1.0.0> ;
                                                        <http://purl.org/dc/terms/creator> "√Ålvaro Carrera Barroso"@en ;
                                                        <http://purl.org/dc/terms/description> "AMOR Experiments is an ontology designed for representing experiments and evaluations in the AMOR project."@en ;
                                                        <http://purl.org/dc/terms/publisher> <http://www.gsi.upm.es> ;
                                                        <http://purl.org/dc/terms/title> "AMOR Experiments Ontology"@en ;
                                                        <http://purl.org/vocab/vann/preferredNamespacePrefix> "amor-exp" ;
                                                        <http://purl.org/vocab/vann/preferredNamespaceUri> "http://www.gsi.upm.es/ontologies/amor/experiments/ns#" ;
                                                        rdfs:comment "AMOR Experiments is an ontology designed for representing experiments and evaluations in the AMOR project."@en ;
                                                        rdfs:label "AMOR Experiments Ontology"@en ;
                                                        owl:versionInfo "1.0.0" .

#################################################################
#    Annotation properties
#################################################################

###  http://purl.org/dc/terms/creator
<http://purl.org/dc/terms/creator> rdf:type owl:AnnotationProperty .


###  http://purl.org/dc/terms/description
<http://purl.org/dc/terms/description> rdf:type owl:AnnotationProperty .


###  http://purl.org/dc/terms/publisher
<http://purl.org/dc/terms/publisher> rdf:type owl:AnnotationProperty .


###  http://purl.org/dc/terms/title
<http://purl.org/dc/terms/title> rdf:type owl:AnnotationProperty .


###  http://purl.org/vocab/vann/preferredNamespacePrefix
<http://purl.org/vocab/vann/preferredNamespacePrefix> rdf:type owl:AnnotationProperty .


###  http://purl.org/vocab/vann/preferredNamespaceUri
<http://purl.org/vocab/vann/preferredNamespaceUri> rdf:type owl:AnnotationProperty .


###  http://schema.org/text
<http://schema.org/text> rdf:type owl:AnnotationProperty .


#################################################################
#    Object Properties
#################################################################

###  http://schema.org/category
<http://schema.org/category> rdf:type owl:ObjectProperty .


###  http://schema.org/hasPart
<http://schema.org/hasPart> rdf:type owl:ObjectProperty .


###  http://schema.org/suggestedAnswer
<http://schema.org/suggestedAnswer> rdf:type owl:ObjectProperty .


###  http://www.gsi.upm.es/ontologies/amor/experiments/ns#hasBackgroundScenario
:hasBackgroundScenario rdf:type owl:ObjectProperty ;
                       rdfs:subPropertyOf :hasParameter ;
                       rdfs:domain :Experiment .


###  http://www.gsi.upm.es/ontologies/amor/experiments/ns#hasContentAdaptationStrategy
:hasContentAdaptationStrategy rdf:type owl:ObjectProperty ;
                              rdfs:subPropertyOf :hasParameter ;
                              rdfs:domain :Experiment ;
                              rdfs:range :ContentAdaptationStrategy ;
                              rdfs:comment "Relates an experiment with the content adaptation strategy used."@en ;
                              rdfs:label "has content adaptation strategy"@en .


###  http://www.gsi.upm.es/ontologies/amor/experiments/ns#hasExecutor
:hasExecutor rdf:type owl:ObjectProperty ;
             rdfs:domain :Experiment ;
             rdfs:range :ExperimentExecutor ;
             rdfs:comment "Relates an experiment with its executor."@en ;
             rdfs:label "has experiment executor"@en .


###  http://www.gsi.upm.es/ontologies/amor/experiments/ns#hasExperimentEvaluation
:hasExperimentEvaluation rdf:type owl:ObjectProperty ;
                         rdfs:subPropertyOf :hasParameter ;
                         rdfs:domain :Experiment ;
                         rdfs:range :ExperimentEvaluation ;
                         rdfs:comment "Relates an experiment with its evaluation."@en ;
                         rdfs:label "has experiment evaluation"@en .


###  http://www.gsi.upm.es/ontologies/amor/experiments/ns#hasExperimentationSubject
:hasExperimentationSubject rdf:type owl:ObjectProperty ;
                           rdfs:domain :Experiment ;
                           rdfs:range :ExperimentionSubject ;
                           rdfs:comment "Relates an experiment with its subject."@en ;
                           rdfs:label "has experimentation subject"@en .


###  http://www.gsi.upm.es/ontologies/amor/experiments/ns#hasFacialExpresivity
:hasFacialExpresivity rdf:type owl:ObjectProperty ;
                      rdfs:domain :Avatar ;
                      rdfs:range :ExpresivityCategory ;
                      rdfs:comment "Relates a character with its facial expresivity."@en ;
                      rdfs:label "has facial expresivity"@en .


###  http://www.gsi.upm.es/ontologies/amor/experiments/ns#hasFinalQuestion
:hasFinalQuestion rdf:type owl:ObjectProperty ;
                  rdfs:domain :ExperimentEvaluation ;
                  rdfs:range <http://schema.org/Question> ;
                  rdfs:comment "Relates an experiment evaluation with the final questionnaire."@en ;
                  rdfs:label "has final question"@en .


###  http://www.gsi.upm.es/ontologies/amor/experiments/ns#hasGesturalExpresivity
:hasGesturalExpresivity rdf:type owl:ObjectProperty ;
                        rdfs:domain :Avatar ;
                        rdfs:range :ExpresivityCategory ;
                        rdfs:comment "Relates a character with its gestural expresivity."@en ;
                        rdfs:label "has gestural expresivity"@en .


###  http://www.gsi.upm.es/ontologies/amor/experiments/ns#hasInitialQuestion
:hasInitialQuestion rdf:type owl:ObjectProperty ;
                    rdfs:domain :ExperimentEvaluation ;
                    rdfs:range <http://schema.org/Question> ;
                    rdfs:comment "Relates an experiment evaluation with the initial questionnaire."@en ;
                    rdfs:label "has initial question"@en .


###  http://www.gsi.upm.es/ontologies/amor/experiments/ns#hasIntermediateQuestion
:hasIntermediateQuestion rdf:type owl:ObjectProperty ;
                         rdfs:domain :ExperimentEvaluation ;
                         rdfs:range <http://schema.org/Question> ;
                         rdfs:comment "Relates an experiment evaluation with the intermediate questionnaire."@en ;
                         rdfs:label "has intermediate question"@en .


###  http://www.gsi.upm.es/ontologies/amor/experiments/ns#hasLLMConfiguration
:hasLLMConfiguration rdf:type owl:ObjectProperty ;
                     rdfs:subPropertyOf :hasParameter ;
                     rdfs:domain :Experiment ;
                     rdfs:range :LLMConfiguration ;
                     rdfs:comment "Relates an experiment with the LLM configuration used."@en ;
                     rdfs:label "has LLM configuration"@en .


###  http://www.gsi.upm.es/ontologies/amor/experiments/ns#hasNews
:hasNews rdf:type owl:ObjectProperty ;
         rdfs:subPropertyOf <http://schema.org/hasPart> ;
         rdfs:domain :NewsDataset ;
         rdfs:range <http://schema.org/NewsArticle> ;
         rdfs:comment "Relates a news dataset with its main entity."@en ;
         rdfs:label "has main entity"@en .


###  http://www.gsi.upm.es/ontologies/amor/experiments/ns#hasParameter
:hasParameter rdf:type owl:ObjectProperty ;
              rdfs:domain :Experiment ;
              rdfs:range owl:Thing ;
              rdfs:comment "Relates an experiment with its parameters."@en ;
              rdfs:label "has parameter"@en .


###  http://www.gsi.upm.es/ontologies/amor/experiments/ns#hasParameterValue
:hasParameterValue rdf:type owl:ObjectProperty .


###  http://www.gsi.upm.es/ontologies/amor/experiments/ns#hasPhysicalMovement
:hasPhysicalMovement rdf:type owl:ObjectProperty ;
                     rdfs:subPropertyOf :hasParameter ;
                     rdfs:domain :Experiment .


###  http://www.gsi.upm.es/ontologies/amor/experiments/ns#hasPreferredContent
:hasPreferredContent rdf:type owl:ObjectProperty ;
                     rdfs:domain :ExperimentionSubject ;
                     rdfs:range <http://schema.org/CreativeWork> ;
                     rdfs:comment "Relates an experimentation subject with its preferred content."@en ;
                     rdfs:label "has preferred content"@en .


###  http://www.gsi.upm.es/ontologies/amor/experiments/ns#hasPreferredEntity
:hasPreferredEntity rdf:type owl:ObjectProperty ;
                    rdfs:domain :ExperimentionSubject ;
                    rdfs:range <http://www.w3.org/ns/prov#Entity> .


###  http://www.gsi.upm.es/ontologies/amor/experiments/ns#hasRecommendationCriterion
:hasRecommendationCriterion rdf:type owl:ObjectProperty ;
                            rdfs:subPropertyOf <http://schema.org/category> ;
                            rdfs:domain :Recommendation ;
                            rdfs:range :RecommendationCriterion ;
                            rdfs:comment "Relates a recommendation with its recommendation criterion."@en ;
                            rdfs:label "has recommendation criterion"@en .


###  http://www.gsi.upm.es/ontologies/amor/experiments/ns#hasRecommendationStrategy
:hasRecommendationStrategy rdf:type owl:ObjectProperty ;
                           rdfs:subPropertyOf :hasParameterValue ;
                           rdfs:domain :RecommendationStrategyParameter ;
                           rdfs:range :RecommendationCriterion ;
                           rdfs:comment "Relates a recommendation strategy parameter with its recommentation strategy."@en ;
                           rdfs:label "has recommendation strategy"@en .


###  http://www.gsi.upm.es/ontologies/amor/experiments/ns#hasRequester
:hasRequester rdf:type owl:ObjectProperty ;
              rdfs:domain :Experiment ;
              rdfs:range :ExperimentRequester ;
              rdfs:comment "Relates an experiment with its requester, i.e. the person who requests the execution of the experiment."@en ;
              rdfs:label "has experiment requester"@en .


###  http://www.gsi.upm.es/ontologies/amor/experiments/ns#hasRobotActor
:hasRobotActor rdf:type owl:ObjectProperty ;
               rdfs:domain :RobotRole ;
               rdfs:range <http://kb.openrobots.org#Robot> .


###  http://www.gsi.upm.es/ontologies/amor/experiments/ns#hasRobotRole
:hasRobotRole rdf:type owl:ObjectProperty ;
              rdfs:domain :RobotCooperationConfiguration ;
              rdfs:range :RobotRole .


###  http://www.gsi.upm.es/ontologies/amor/experiments/ns#hasVisualizationStrategy
:hasVisualizationStrategy rdf:type owl:ObjectProperty ;
                          rdfs:subPropertyOf :hasParameter ;
                          rdfs:domain :Experiment ;
                          rdfs:range :VisualizationStrategy ;
                          rdfs:comment "Relates an experiment with its visualization strategy."@en ;
                          rdfs:label "has visualization strategy"@en .


###  http://www.gsi.upm.es/ontologies/amor/experiments/ns#hasVocalExpresivity
:hasVocalExpresivity rdf:type owl:ObjectProperty ;
                     rdfs:domain :Avatar ;
                     rdfs:range :ExpresivityCategory ;
                     rdfs:comment "Relates a character with its vocal expresivity."@en ;
                     rdfs:label "has vocal expresivity"@en .


###  http://www.gsi.upm.es/ontologies/amor/experiments/ns#isRelatedWithExperiment
:isRelatedWithExperiment rdf:type owl:ObjectProperty ;
                         rdfs:subPropertyOf <http://www.w3.org/ns/prov#wasAssociatedWith> ;
                         rdfs:domain <http://www.gsi.upm.es/ontologies/segb/ns#LoggedActivity> ;
                         rdfs:range :Experiment ;
                         rdfs:comment "Relates an activity logged in the AMOR-SEGB with the experiment in progress."@en ;
                         rdfs:label "is related with experiment"@en .


###  http://www.gsi.upm.es/ontologies/amor/experiments/ns#usesAggregatedData
:usesAggregatedData rdf:type owl:ObjectProperty ;
                    rdfs:subPropertyOf :hasParameter ;
                    rdfs:domain :Experiment .


###  http://www.gsi.upm.es/ontologies/amor/experiments/ns#usesAvatar
:usesAvatar rdf:type owl:ObjectProperty ;
            rdfs:subPropertyOf :hasParameter ;
            rdfs:domain :Experiment ;
            rdfs:range :Avatar ;
            rdfs:comment "Relates an experiment with the avatar used."@en ;
            rdfs:label "uses avatar"@en .


###  http://www.gsi.upm.es/ontologies/amor/experiments/ns#usesDataset
:usesDataset rdf:type owl:ObjectProperty ;
             rdfs:subPropertyOf :hasParameter ;
             rdfs:domain :DigitalNewspaperExperiment ;
             rdfs:range :NewsDataset ;
             rdfs:comment "Relates a news content dataset parameter with its dataset."@en ;
             rdfs:label "has dataset"@en .


###  http://www.gsi.upm.es/ontologies/amor/experiments/ns#usesEmotionRecognitionCooperationStrategy
:usesEmotionRecognitionCooperationStrategy rdf:type owl:ObjectProperty ;
                                           rdfs:subPropertyOf :hasParameter ;
                                           rdfs:domain :Experiment ;
                                           rdfs:range :EmotionRecognitionCooperationStrategy ;
                                           rdfs:comment "Relates an experiment with the emotion recognition cooperation configuration used."@en ;
                                           rdfs:label "uses emotion recognition cooperation configuration"@en .


###  http://www.gsi.upm.es/ontologies/amor/experiments/ns#usesLanguage
:usesLanguage rdf:type owl:ObjectProperty ;
              rdfs:subPropertyOf :hasParameter ;
              rdfs:domain :Experiment ;
              rdfs:range <http://www.w3.org/XML/1998/namespace/lang> .


###  http://www.gsi.upm.es/ontologies/amor/experiments/ns#usesRobotCooperationConfiguration
:usesRobotCooperationConfiguration rdf:type owl:ObjectProperty ;
                                   rdfs:subPropertyOf :hasParameter ;
                                   rdfs:domain :Experiment ;
                                   rdfs:range :RobotCooperationConfiguration ;
                                   rdfs:comment "Relates an experiment with the robot cooperation configuration used."@en ;
                                   rdfs:label "uses robot cooperation configuration"@en .


###  http://www.gsi.upm.es/ontologies/amor/experiments/ns#usesRobotCooperationStrategy
:usesRobotCooperationStrategy rdf:type owl:ObjectProperty ;
                              rdfs:subPropertyOf :hasParameter ;
                              rdfs:domain :RobotCooperationConfiguration ;
                              rdfs:range :RobotCooperationStrategy ;
                              rdfs:comment "Relates a robot cooperation configuration with the robot cooperation strategy used."@en ;
                              rdfs:label "uses robot cooperation strategy"@en .


###  http://www.gsi.upm.es/ontologies/amor/experiments/ns#usesSemanticCooperationConfiguration
:usesSemanticCooperationConfiguration rdf:type owl:ObjectProperty ;
                                      rdfs:subPropertyOf :hasParameter ;
                                      rdfs:domain :Experiment ;
                                      rdfs:range :SemanticCooperationConfiguration ;
                                      rdfs:comment "Relates an experiment with the semantic cooperation strategy used."@en ;
                                      rdfs:label "uses semantic cooperation strategy"@en .


###  http://www.gsi.upm.es/ontologies/amor/experiments/ns#usesSemanticCooperationStrategy
:usesSemanticCooperationStrategy rdf:type owl:ObjectProperty ;
                                 rdfs:subPropertyOf :hasParameter ;
                                 rdfs:domain :SemanticCooperationConfiguration ;
                                 rdfs:range :SemanticCooperationStrategy ;
                                 rdfs:comment "Relates an experiment with the semantic cooperation strategy used."@en ;
                                 rdfs:label "uses semantic cooperation strategy"@en .


###  http://www.w3.org/ns/prov#wasAssociatedWith
<http://www.w3.org/ns/prov#wasAssociatedWith> rdf:type owl:ObjectProperty .


#################################################################
#    Data properties
#################################################################

###  http://www.gsi.upm.es/ontologies/amor/experiments/ns#hasAccesibilityCategory
:hasAccesibilityCategory rdf:type owl:DatatypeProperty ;
                         rdfs:domain :ExperimentionSubject ;
                         rdfs:range xsd:string ;
                         rdfs:comment "Relates an experimentation subject with its accesibility category."@en ;
                         rdfs:label "has accesibility category"@en .


###  http://www.gsi.upm.es/ontologies/amor/experiments/ns#hasAgeBracket
:hasAgeBracket rdf:type owl:DatatypeProperty ;
               rdfs:domain :ExperimentionSubject ;
               rdfs:range xsd:string ;
               rdfs:comment "Relates an experimentation subject with its age bracket."@en ;
               rdfs:label "has age bracket"@en .


###  http://www.gsi.upm.es/ontologies/amor/experiments/ns#hasAppearance
:hasAppearance rdf:type owl:DatatypeProperty ;
               rdfs:domain :Avatar ;
               rdfs:range xsd:string ;
               rdfs:comment "Relates a character with its appearance."@en ;
               rdfs:label "has appearance"@en .


###  http://www.gsi.upm.es/ontologies/amor/experiments/ns#hasAverageSocialNetworkActivityPerMonth
:hasAverageSocialNetworkActivityPerMonth rdf:type owl:DatatypeProperty ;
                                         rdfs:domain :ExperimentionSubject ;
                                         rdfs:range xsd:integer ;
                                         rdfs:comment "Relates an experimentation subject with the average social network activity per month."@en ;
                                         rdfs:label "has average social network activity per month"@en .


###  http://www.gsi.upm.es/ontologies/amor/experiments/ns#hasBackgroundMusic
:hasBackgroundMusic rdf:type owl:DatatypeProperty ;
                    rdfs:domain :Experiment ;
                    rdfs:range xsd:string ;
                    rdfs:comment "Relates an experiment with the background music used."@en ;
                    rdfs:label "has background music"@en .


###  http://www.gsi.upm.es/ontologies/amor/experiments/ns#hasBackgroundScenario
:hasBackgroundScenario rdf:type owl:DatatypeProperty ;
                       rdfs:range xsd:string .


###  http://www.gsi.upm.es/ontologies/amor/experiments/ns#hasCategory
:hasCategory rdf:type owl:DatatypeProperty ;
             rdfs:domain :Avatar ;
             rdfs:range xsd:string ;
             rdfs:comment "Relates a character with its category."@en ;
             rdfs:label "has category"@en .


###  http://www.gsi.upm.es/ontologies/amor/experiments/ns#hasEducationalLevel
:hasEducationalLevel rdf:type owl:DatatypeProperty ;
                     rdfs:domain :ExperimentionSubject ;
                     rdfs:range xsd:string ;
                     rdfs:comment "Relates an experimentation subject with its educational level."@en ;
                     rdfs:label "has educational level"@en .


###  http://www.gsi.upm.es/ontologies/amor/experiments/ns#hasLLMToken
:hasLLMToken rdf:type owl:DatatypeProperty ;
             rdfs:domain :LLMConfiguration ;
             rdfs:range xsd:string ;
             rdfs:comment "Relates an LLM configuration with the LLM token used."@en ;
             rdfs:label "has LLM token"@en .


###  http://www.gsi.upm.es/ontologies/amor/experiments/ns#hasLanguageComplexityLevel
:hasLanguageComplexityLevel rdf:type owl:DatatypeProperty ;
                            rdfs:domain :Avatar ;
                            rdfs:range xsd:string ;
                            rdfs:comment "Relates a character with its language complexity level."@en ;
                            rdfs:label "has language complexity level"@en .


###  http://www.gsi.upm.es/ontologies/amor/experiments/ns#hasNumberOfFollowers
:hasNumberOfFollowers rdf:type owl:DatatypeProperty ;
                      rdfs:domain :ExperimentionSubject ;
                      rdfs:range xsd:integer ;
                      rdfs:comment "Relates an experimentation subject with the number of followers."@en ;
                      rdfs:label "has number of followers"@en .


###  http://www.gsi.upm.es/ontologies/amor/experiments/ns#hasPersonality
:hasPersonality rdf:type owl:DatatypeProperty ;
                rdfs:domain :Avatar ;
                rdfs:range xsd:string ;
                rdfs:comment "Relates a character with its personality."@en ;
                rdfs:label "has personality"@en .


###  http://www.gsi.upm.es/ontologies/amor/experiments/ns#hasPhysicalMovement
:hasPhysicalMovement rdf:type owl:DatatypeProperty ;
                     rdfs:range xsd:string .


###  http://www.gsi.upm.es/ontologies/amor/experiments/ns#hasPoliticalOrientation
:hasPoliticalOrientation rdf:type owl:DatatypeProperty ;
                         rdfs:domain :ExperimentionSubject ;
                         rdfs:range xsd:string ;
                         rdfs:comment "Relates an experimentation subject with its political orientation."@en ;
                         rdfs:label "has political orientation"@en .


###  http://www.gsi.upm.es/ontologies/amor/experiments/ns#hasPreferredEntity
:hasPreferredEntity rdf:type owl:DatatypeProperty .


###  http://www.gsi.upm.es/ontologies/amor/experiments/ns#hasPreferredTopic
:hasPreferredTopic rdf:type owl:DatatypeProperty ;
                   rdfs:domain :ExperimentionSubject ;
                   rdfs:range xsd:string ;
                   rdfs:comment "Relates an experimentation subject with its preferred topic."@en ;
                   rdfs:label "has preferred topic"@en .


###  http://www.gsi.upm.es/ontologies/amor/experiments/ns#hasRecommendationScore
:hasRecommendationScore rdf:type owl:DatatypeProperty ;
                        rdfs:domain :Recommendation ;
                        rdfs:range xsd:float ;
                        rdfs:comment "Relates a recommendation with the score of the recommendation."@en ;
                        rdfs:label "has recommendation score"@en .


###  http://www.gsi.upm.es/ontologies/amor/experiments/ns#hasRobotActor
:hasRobotActor rdf:type owl:DatatypeProperty .


###  http://www.gsi.upm.es/ontologies/amor/experiments/ns#hasRobotRole
:hasRobotRole rdf:type owl:DatatypeProperty .


###  http://www.gsi.upm.es/ontologies/amor/experiments/ns#hasRoleType
:hasRoleType rdf:type owl:DatatypeProperty ;
             rdfs:domain :RobotRole ;
             rdfs:range xsd:string ;
             rdfs:comment "Relates a robot role with the robot role type."@en ;
             rdfs:label "has robot role type"@en .


###  http://www.gsi.upm.es/ontologies/amor/experiments/ns#hasStressLevel
:hasStressLevel rdf:type owl:DatatypeProperty ;
                rdfs:domain :ExperimentionSubject ;
                rdfs:range xsd:float ;
                rdfs:comment "Relates an experimentation subject with its stress level (between 0.0 to 1.0)."@en ;
                rdfs:label "has stress level"@en .


###  http://www.gsi.upm.es/ontologies/amor/experiments/ns#hasVoice
:hasVoice rdf:type owl:DatatypeProperty ;
          rdfs:domain :Avatar ;
          rdfs:range xsd:string ;
          rdfs:comment "Relates a character with its voice."@en ;
          rdfs:label "has voice"@en .


###  http://www.gsi.upm.es/ontologies/amor/experiments/ns#usesAggregatedData
:usesAggregatedData rdf:type owl:DatatypeProperty ;
                    rdfs:range xsd:string .


###  http://www.gsi.upm.es/ontologies/amor/experiments/ns#usesCloudGraphQuery
:usesCloudGraphQuery rdf:type owl:DatatypeProperty ;
                     rdfs:domain :SemanticCooperationConfiguration ;
                     rdfs:range xsd:string ;
                     rdfs:comment "Relates a semantic cooperation strategy with the cloud graph query used."@en ;
                     rdfs:label "uses cloud graph query"@en .


###  http://www.gsi.upm.es/ontologies/amor/experiments/ns#usesLLMEndPoint
:usesLLMEndPoint rdf:type owl:DatatypeProperty ;
                 rdfs:domain :LLMConfiguration ;
                 rdfs:range xsd:string ;
                 rdfs:comment "Relates an LLM configuration with the LLM end point used."@en ;
                 rdfs:label "uses LLM end point"@en .


###  http://www.gsi.upm.es/ontologies/amor/experiments/ns#usesLLMModel
:usesLLMModel rdf:type owl:DatatypeProperty ;
              rdfs:domain :LLMConfiguration ;
              rdfs:range xsd:string ;
              rdfs:comment "Relates an LLM configuration with the LLM model used."@en ;
              rdfs:label "uses LLM model"@en .


###  http://www.gsi.upm.es/ontologies/amor/experiments/ns#usesLLMService
:usesLLMService rdf:type owl:DatatypeProperty ;
                rdfs:domain :LLMConfiguration ;
                rdfs:range xsd:string ;
                rdfs:comment "Relates an LLM configuration with the LLM service used."@en ;
                rdfs:label "uses LLM service"@en .


###  http://www.gsi.upm.es/ontologies/amor/experiments/ns#usesLanguage
:usesLanguage rdf:type owl:DatatypeProperty .


###  http://www.gsi.upm.es/ontologies/amor/experiments/ns#usesPrompt
:usesPrompt rdf:type owl:DatatypeProperty ;
            rdfs:domain :LLMConfiguration ;
            rdfs:range xsd:string ;
            rdfs:comment "Relates an LLM configuration with the prompt used."@en ;
            rdfs:label "uses prompt"@en .


###  http://www.gsi.upm.es/ontologies/amor/experiments/ns#usesSPARQLQuery
:usesSPARQLQuery rdf:type owl:DatatypeProperty ;
                 rdfs:domain :SemanticCooperationConfiguration ;
                 rdfs:range xsd:string ;
                 rdfs:comment "Relates a semantic cooperation strategy with the SPARQL query used."@en ;
                 rdfs:label "uses SPARQL query"@en .


#################################################################
#    Classes
#################################################################

###  http://kb.openrobots.org#Robot
<http://kb.openrobots.org#Robot> rdf:type owl:Class .


###  http://schema.org/Answer
<http://schema.org/Answer> rdf:type owl:Class .


###  http://schema.org/CreativeWork
<http://schema.org/CreativeWork> rdf:type owl:Class .


###  http://schema.org/Dataset
<http://schema.org/Dataset> rdf:type owl:Class .


###  http://schema.org/NewsArticle
<http://schema.org/NewsArticle> rdf:type owl:Class .


###  http://schema.org/Question
<http://schema.org/Question> rdf:type owl:Class .


###  http://www.gsi.upm.es/ontologies/amor/experiments/ns#Avatar
:Avatar rdf:type owl:Class ;
        rdfs:subClassOf <http://xmlns.com/foaf/0.1/Agent> ;
        rdfs:comment "Represents an avatar used in an experiment in the AMOR project."@en ;
        rdfs:label "Avatar"@en .


###  http://www.gsi.upm.es/ontologies/amor/experiments/ns#ClickBaitExperiment
:ClickBaitExperiment rdf:type owl:Class ;
                     rdfs:subClassOf :DigitalNewspaperExperiment ;
                     rdfs:comment "Represents an experiment with click bait in the AMOR project."@en ;
                     rdfs:label "Click Bait Experiment"@en .


###  http://www.gsi.upm.es/ontologies/amor/experiments/ns#ContentAdaptationStrategy
:ContentAdaptationStrategy rdf:type owl:Class ;
                           rdfs:comment "Represents a strategy used to adapt the content in an experiment in the AMOR project."@en ;
                           rdfs:label "Content Adaptation Strategy"@en .


###  http://www.gsi.upm.es/ontologies/amor/experiments/ns#DigitalNewspaperExperiment
:DigitalNewspaperExperiment rdf:type owl:Class ;
                            rdfs:subClassOf :Experiment ;
                            rdfs:comment "Represents an experiment with a digital newspaper in the AMOR project."@en ;
                            rdfs:label "Digital Newspaper Experiment"@en .


###  http://www.gsi.upm.es/ontologies/amor/experiments/ns#EmotionRecognitionCooperationStrategy
:EmotionRecognitionCooperationStrategy rdf:type owl:Class ;
                                       rdfs:comment "Represents the strategy used to cooperate with the emotion recognition in an experiment in the AMOR project."@en ;
                                       rdfs:label "Emotion Recognition Cooperation Strategy"@en .


###  http://www.gsi.upm.es/ontologies/amor/experiments/ns#Experiment
:Experiment rdf:type owl:Class ;
            rdfs:subClassOf <http://www.w3.org/ns/prov#Activity> ;
            rdfs:comment "Represents an experiment in the AMOR project."@en ;
            rdfs:label "Experiment"@en .


###  http://www.gsi.upm.es/ontologies/amor/experiments/ns#ExperimentEvaluation
:ExperimentEvaluation rdf:type owl:Class ;
                      rdfs:subClassOf <http://www.w3.org/ns/prov#Entity> ;
                      rdfs:comment "Represents an evaluation of an experiment in the AMOR project."@en ;
                      rdfs:label "Experiment Evaluation"@en .


###  http://www.gsi.upm.es/ontologies/amor/experiments/ns#ExperimentExecutor
:ExperimentExecutor rdf:type owl:Class ;
                    rdfs:subClassOf <http://www.w3.org/ns/prov#Agent> ;
                    rdfs:comment "Represents an executor of an experiment in the AMOR project."@en ;
                    rdfs:label "Experiment Executor"@en .


###  http://www.gsi.upm.es/ontologies/amor/experiments/ns#ExperimentParameter
:ExperimentParameter rdf:type owl:Class ;
                     rdfs:subClassOf <http://www.w3.org/ns/prov#Entity> ;
                     rdfs:comment "Represents a parameter of an experiment in the AMOR project."@en ;
                     rdfs:label "Experiment Parameter"@en .


###  http://www.gsi.upm.es/ontologies/amor/experiments/ns#ExperimentRequester
:ExperimentRequester rdf:type owl:Class ;
                     rdfs:subClassOf <http://www.w3.org/ns/prov#Agent> ;
                     rdfs:comment "Represents a requester of an experiment in the AMOR project."@en ;
                     rdfs:label "Experiment Requester"@en .


###  http://www.gsi.upm.es/ontologies/amor/experiments/ns#ExperimentationSubject
:ExperimentationSubject rdf:type owl:Class ;
                        rdfs:subClassOf <http://www.w3.org/ns/prov#Agent> ;
                        rdfs:comment "Represents a subject of an experiment in the AMOR project."@en ;
                        rdfs:label "Experimentation Subject"@en .


###  http://www.gsi.upm.es/ontologies/amor/experiments/ns#ExperimentionSubject
:ExperimentionSubject rdf:type owl:Class .


###  http://www.gsi.upm.es/ontologies/amor/experiments/ns#ExpresivityCategory
:ExpresivityCategory rdf:type owl:Class ;
                     rdfs:comment "Represents the expresivity category of a character in an experiment in the AMOR project."@en ;
                     rdfs:label "Expresivity Category"@en .


###  http://www.gsi.upm.es/ontologies/amor/experiments/ns#FakeNewsAwarenessExperiment
:FakeNewsAwarenessExperiment rdf:type owl:Class ;
                             rdfs:subClassOf :DigitalNewspaperExperiment ;
                             rdfs:comment "Represents an experiment with fake news awareness in the AMOR project."@en ;
                             rdfs:label "Fake News Awareness Experiment"@en .


###  http://www.gsi.upm.es/ontologies/amor/experiments/ns#GeographicalVisualizationExperiment
:GeographicalVisualizationExperiment rdf:type owl:Class ;
                                     rdfs:subClassOf :Experiment ;
                                     rdfs:comment "Represents an experiment with geographical visualization in the AMOR project."@en ;
                                     rdfs:label "Geographical Visualization Experiment"@en .


###  http://www.gsi.upm.es/ontologies/amor/experiments/ns#LLMConfiguration
:LLMConfiguration rdf:type owl:Class ;
                  rdfs:comment "Represents the configuration of the LLM used in an experiment in the AMOR project."@en ;
                  rdfs:label "LLM Configuration"@en .


###  http://www.gsi.upm.es/ontologies/amor/experiments/ns#LikertQuestion
:LikertQuestion rdf:type owl:Class ;
                rdfs:subClassOf <http://schema.org/Question> ,
                                [ rdf:type owl:Restriction ;
                                  owl:onProperty <http://schema.org/suggestedAnswer> ;
                                  owl:allValuesFrom [ rdf:type owl:Class ;
                                                      owl:unionOf ( [ rdf:type owl:Restriction ;
                                                                      owl:onProperty <http://schema.org/suggestedAnswer> ;
                                                                      owl:allValuesFrom [ rdf:type owl:Class ;
                                                                                          owl:oneOf ( _:genid28 rdf:type <http://schema.org/Answer> ;
                                                                                                                <http://schema.org/text> "Strongly Disagree"
                                                                                                    _:genid26 rdf:type <http://schema.org/Answer> ;
                                                                                                              <http://schema.org/text> "Disagree"
                                                                                                    _:genid24 rdf:type <http://schema.org/Answer> ;
                                                                                                              <http://schema.org/text> "Neutral"
                                                                                                    _:genid22 rdf:type <http://schema.org/Answer> ;
                                                                                                              <http://schema.org/text> "Agree"
                                                                                          _:genid20 rdf:type <http://schema.org/Answer> ;
                                                                                                    <http://schema.org/text> "Strongly Agree"
                                                                                        )
                                                                    ]
                                                                  ]
                                                    [ rdf:type owl:Restriction ;
                                                      owl:onProperty <http://schema.org/suggestedAnswer> ;
                                                      owl:allValuesFrom [ rdf:type owl:Class ;
                                                                          owl:oneOf ( _:genid15 rdf:type <http://schema.org/Answer> ;
                                                                                                <http://schema.org/text> "1"
                                                                                    _:genid13 rdf:type <http://schema.org/Answer> ;
                                                                                              <http://schema.org/text> "2"
                                                                                    _:genid11 rdf:type <http://schema.org/Answer> ;
                                                                                              <http://schema.org/text> "3"
                                                                                    _:genid9 rdf:type <http://schema.org/Answer> ;
                                                                                             <http://schema.org/text> "4"
                                                                          _:genid7 rdf:type <http://schema.org/Answer> ;
                                                                                   <http://schema.org/text> "5"
                                                                        )
                                                    ]
                                  ]
                                )
]
] ;
rdfs:comment "Represents a Likert question."@en ;
rdfs:label "Likert Question"@en .


###  http://www.gsi.upm.es/ontologies/amor/experiments/ns#MoralFrameExperiment
:MoralFrameExperiment rdf:type owl:Class ;
                      rdfs:subClassOf :DigitalNewspaperExperiment ;
                      rdfs:comment "Represents an experiment with a moral frame in the AMOR project."@en ;
                      rdfs:label "Moral Frame Experiment"@en .


###  http://www.gsi.upm.es/ontologies/amor/experiments/ns#MoralValuesExperiment
:MoralValuesExperiment rdf:type owl:Class ;
                       rdfs:subClassOf :DigitalNewspaperExperiment ;
                       rdfs:comment "Represents an experiment with moral values in the AMOR project."@en ;
                       rdfs:label "Moral Values Experiment"@en .


###  http://www.gsi.upm.es/ontologies/amor/experiments/ns#NewsDataset
:NewsDataset rdf:type owl:Class ;
             rdfs:subClassOf <http://schema.org/Dataset> ,
                             :ExperimentParameter ;
             rdfs:comment "Represents a dataset of news content."@en ;
             rdfs:label "News Dataset"@en .


###  http://www.gsi.upm.es/ontologies/amor/experiments/ns#Recommendation
:Recommendation rdf:type owl:Class ;
                rdfs:subClassOf <http://www.w3.org/ns/oa#Recommendation> ;
                rdfs:comment "Represents a recommendation for a piee of content."@en ;
                rdfs:label "Recommendation"@en .


###  http://www.gsi.upm.es/ontologies/amor/experiments/ns#RecommendationCriterion
:RecommendationCriterion rdf:type owl:Class ;
                         rdfs:comment "Represents a criterion used to filter recommendations in an experiment in the AMOR project."@en ;
                         rdfs:label "Recommendation Criterion"@en .


###  http://www.gsi.upm.es/ontologies/amor/experiments/ns#RecommendationStrategyParameter
:RecommendationStrategyParameter rdf:type owl:Class ;
                                 rdfs:subClassOf :ExperimentParameter ;
                                 rdfs:comment "Represents the strategy used to filter recommendations for an item in an experiment in the AMOR project."@en ;
                                 rdfs:label "Recommendation Strategy Parameter"@en .


###  http://www.gsi.upm.es/ontologies/amor/experiments/ns#RobotCooperationConfiguration
:RobotCooperationConfiguration rdf:type owl:Class .


###  http://www.gsi.upm.es/ontologies/amor/experiments/ns#RobotCooperationStrategy
:RobotCooperationStrategy rdf:type owl:Class ;
                          rdfs:comment "Represents the strategy used to cooperate with the robot in an experiment in the AMOR project."@en ;
                          rdfs:label "Robot Cooperation Strategy"@en .


###  http://www.gsi.upm.es/ontologies/amor/experiments/ns#RobotRole
:RobotRole rdf:type owl:Class ;
           rdfs:comment "Represents the role of a robot in an experiment in the AMOR project."@en ;
           rdfs:label "Robot Role"@en .


###  http://www.gsi.upm.es/ontologies/amor/experiments/ns#SearchEngineBiasExperiment
:SearchEngineBiasExperiment rdf:type owl:Class ;
                            rdfs:subClassOf :DigitalNewspaperExperiment ;
                            rdfs:comment "Represents an experiment with a search engine bias in the AMOR project."@en ;
                            rdfs:label "Search Engine Bias Experiment"@en .


###  http://www.gsi.upm.es/ontologies/amor/experiments/ns#SemanticCooperationConfiguration
:SemanticCooperationConfiguration rdf:type owl:Class ;
                                  rdfs:comment "Represents the configuration of the semantic cooperation used in an experiment in the AMOR project."@en ;
                                  rdfs:label "Semantic Cooperation Configuration"@en .


###  http://www.gsi.upm.es/ontologies/amor/experiments/ns#SemanticCooperationStrategy
:SemanticCooperationStrategy rdf:type owl:Class ;
                             rdfs:comment "Represents the strategy used to cooperate with the semantic web in an experiment in the AMOR project."@en ;
                             rdfs:label "Semantic Cooperation Strategy"@en .


###  http://www.gsi.upm.es/ontologies/amor/experiments/ns#SocialNetworkExperiment
:SocialNetworkExperiment rdf:type owl:Class ;
                         rdfs:subClassOf :Experiment ;
                         rdfs:comment "Represents an experiment with a social network in the AMOR project."@en ;
                         rdfs:label "Social Network Experiment"@en .


###  http://www.gsi.upm.es/ontologies/amor/experiments/ns#VisualizationStrategy
:VisualizationStrategy rdf:type owl:Class ;
                       rdfs:comment "Represents a strategy used to visualize the results of an experiment in the AMOR project."@en ;
                       rdfs:label "Visualization Strategy"@en .


###  http://www.gsi.upm.es/ontologies/segb/ns#LoggedActivity
<http://www.gsi.upm.es/ontologies/segb/ns#LoggedActivity> rdf:type owl:Class .


###  http://www.w3.org/XML/1998/namespace/lang
<http://www.w3.org/XML/1998/namespace/lang> rdf:type owl:Class .


###  http://www.w3.org/ns/oa#Recommendation
<http://www.w3.org/ns/oa#Recommendation> rdf:type owl:Class .


###  http://www.w3.org/ns/prov#Activity
<http://www.w3.org/ns/prov#Activity> rdf:type owl:Class .


###  http://www.w3.org/ns/prov#Agent
<http://www.w3.org/ns/prov#Agent> rdf:type owl:Class .


###  http://www.w3.org/ns/prov#Entity
<http://www.w3.org/ns/prov#Entity> rdf:type owl:Class .


###  http://xmlns.com/foaf/0.1/Agent
<http://xmlns.com/foaf/0.1/Agent> rdf:type owl:Class .


#################################################################
#    Individuals
#################################################################

###  http://www.gsi.upm.es/ontologies/amor/experiments/ns#AfectiveAdaptationStrategy
:AfectiveAdaptationStrategy rdf:type owl:NamedIndividual ,
                                     :ContentAdaptationStrategy ;
                            rdfs:comment "Represents the affective adaptation strategy."@en ;
                            rdfs:label "Affective Adaptation Strategy"@en .


###  http://www.gsi.upm.es/ontologies/amor/experiments/ns#AffectiveValueVisualizationStrategy
:AffectiveValueVisualizationStrategy rdf:type owl:NamedIndividual ,
                                              :VisualizationStrategy ;
                                     rdfs:comment "Represents the strategy used to visualize the affective values of the results of an experiment in the AMOR project."@en ;
                                     rdfs:label "Affective Value Visualization Strategy"@en .


###  http://www.gsi.upm.es/ontologies/amor/experiments/ns#ClickBaitVisualizationStrategy
:ClickBaitVisualizationStrategy rdf:type owl:NamedIndividual ,
                                         :VisualizationStrategy ;
                                rdfs:comment "Represents the strategy used to visualize the click bait values of the results of an experiment in the AMOR project."@en ;
                                rdfs:label "Click Bait Visualization Strategy"@en .


###  http://www.gsi.upm.es/ontologies/amor/experiments/ns#CloudEmotionRecognition
:CloudEmotionRecognition rdf:type owl:NamedIndividual ,
                                  :EmotionRecognitionCooperationStrategy ;
                         rdfs:comment "Represents the cloud cooperation in emotion recognition in an experiment."@en ;
                         rdfs:label "Cloud Cooperation Emotion Recognition"@en .


###  http://www.gsi.upm.es/ontologies/amor/experiments/ns#CloudSemanticCooperation
:CloudSemanticCooperation rdf:type owl:NamedIndividual ,
                                   :SemanticCooperationStrategy ;
                          rdfs:comment "Represents the cloud semantic cooperation in an experiment."@en ;
                          rdfs:label "Cloud Semantic Cooperation"@en .


###  http://www.gsi.upm.es/ontologies/amor/experiments/ns#CompetitiveRobot
:CompetitiveRobot rdf:type owl:NamedIndividual ,
                           :RobotCooperationStrategy ;
                  rdfs:comment "Represents the competitive cooperation in robot in an experiment."@en ;
                  rdfs:label "Competitive Cooperation Robot"@en .


###  http://www.gsi.upm.es/ontologies/amor/experiments/ns#CooperativeRobot
:CooperativeRobot rdf:type owl:NamedIndividual ,
                           :RobotCooperationStrategy ;
                  rdfs:comment "Represents the cognitive cooperation in robot in an experiment."@en ;
                  rdfs:label "Cognitive Cooperation Robot"@en .


###  http://www.gsi.upm.es/ontologies/amor/experiments/ns#EmotionDissimilarity
:EmotionDissimilarity rdf:type owl:NamedIndividual ,
                               :RecommendationCriterion ;
                      rdfs:comment "Recommends elements with an opposite emotion value"@en ;
                      rdfs:label "Opposite Emotion Recommendation Strategy"@en .


###  http://www.gsi.upm.es/ontologies/amor/experiments/ns#EmotionSimilarity
:EmotionSimilarity rdf:type owl:NamedIndividual ,
                            :RecommendationCriterion ;
                   rdfs:comment "Recommends elements with a similar emotion value"@en ;
                   rdfs:label "Similar Emotion Recommendation Strategy"@en .


###  http://www.gsi.upm.es/ontologies/amor/experiments/ns#EmotiveExpresivity
:EmotiveExpresivity rdf:type owl:NamedIndividual ,
                             :ExpresivityCategory ;
                    rdfs:comment "Represents the emotive expresivity of a character."@en ;
                    rdfs:label "Emotive Expresivity"@en .


###  http://www.gsi.upm.es/ontologies/amor/experiments/ns#EmphaticExpresivity
:EmphaticExpresivity rdf:type owl:NamedIndividual ,
                              :ExpresivityCategory ;
                     rdfs:comment "Represents the emphatic expresivity of a character."@en ;
                     rdfs:label "Emphatic Expresivity"@en .


###  http://www.gsi.upm.es/ontologies/amor/experiments/ns#EntitySimilarity
:EntitySimilarity rdf:type owl:NamedIndividual ,
                           :RecommendationCriterion ;
                  rdfs:comment "Recommends elements with a similar named entities"@en ;
                  rdfs:label "Similar Entities Recommendation Strategy"@en .


###  http://www.gsi.upm.es/ontologies/amor/experiments/ns#ExaggeratedExpresivity
:ExaggeratedExpresivity rdf:type owl:NamedIndividual ,
                                 :ExpresivityCategory ;
                        rdfs:comment "Represents the exaggerated expresivity of a character."@en ;
                        rdfs:label "Exaggerated Expresivity"@en .


###  http://www.gsi.upm.es/ontologies/amor/experiments/ns#FakeNewsVisualizationStrategy
:FakeNewsVisualizationStrategy rdf:type owl:NamedIndividual ,
                                        :VisualizationStrategy ;
                               rdfs:comment "Represents the strategy used to visualize the fake news values of the results of an experiment in the AMOR project."@en ;
                               rdfs:label "Fake News Visualization Strategy"@en .


###  http://www.gsi.upm.es/ontologies/amor/experiments/ns#FullCooperationEmotionRecognition
:FullCooperationEmotionRecognition rdf:type owl:NamedIndividual ,
                                            :EmotionRecognitionCooperationStrategy ;
                                   rdfs:comment "Represents the full cooperation in emotion recognition in an experiment."@en ;
                                   rdfs:label "Full Cooperation Emotion Recognition"@en .


###  http://www.gsi.upm.es/ontologies/amor/experiments/ns#FullSemanticCooperation
:FullSemanticCooperation rdf:type owl:NamedIndividual ,
                                  :SemanticCooperationStrategy ;
                         rdfs:comment "Represents the full semantic cooperation in an experiment."@en ;
                         rdfs:label "Full Semantic Cooperation"@en .


###  http://www.gsi.upm.es/ontologies/amor/experiments/ns#LocalEmotionRecognition
:LocalEmotionRecognition rdf:type owl:NamedIndividual ,
                                  :EmotionRecognitionCooperationStrategy ;
                         rdfs:comment "Represents the local cooperation in emotion recognition in an experiment."@en ;
                         rdfs:label "Local Cooperation Emotion Recognition"@en .


###  http://www.gsi.upm.es/ontologies/amor/experiments/ns#LocalSemanticCooperation
:LocalSemanticCooperation rdf:type owl:NamedIndividual ,
                                   :SemanticCooperationStrategy ;
                          rdfs:comment "Represents the local semantic cooperation in an experiment."@en ;
                          rdfs:label "Local Semantic Cooperation"@en .


###  http://www.gsi.upm.es/ontologies/amor/experiments/ns#MoralAdaptationStrategy
:MoralAdaptationStrategy rdf:type owl:NamedIndividual ,
                                  :ContentAdaptationStrategy ;
                         rdfs:comment "Represents the moral adaptation strategy."@en ;
                         rdfs:label "Moral Adaptation Strategy"@en .


###  http://www.gsi.upm.es/ontologies/amor/experiments/ns#MoralDissimilarity
:MoralDissimilarity rdf:type owl:NamedIndividual ,
                             :RecommendationCriterion ;
                    rdfs:comment "Recommends elements with an opposite moral value"@en ;
                    rdfs:label "Opposite Moral Recommendation Strategy"@en .


###  http://www.gsi.upm.es/ontologies/amor/experiments/ns#MoralSimilarity
:MoralSimilarity rdf:type owl:NamedIndividual ,
                          :RecommendationCriterion ;
                 rdfs:comment "Recommends elements with a similar moral value"@en ;
                 rdfs:label "Similar Moral Recommendation Strategy"@en .


###  http://www.gsi.upm.es/ontologies/amor/experiments/ns#MoralValueVisualizationStrategy
:MoralValueVisualizationStrategy rdf:type owl:NamedIndividual ,
                                          :VisualizationStrategy ;
                                 rdfs:comment "Represents the strategy used to visualize the moral values of the results of an experiment in the AMOR project."@en ;
                                 rdfs:label "Moral Value Visualization Strategy"@en .


###  http://www.gsi.upm.es/ontologies/amor/experiments/ns#NoAdaptationStrategy
:NoAdaptationStrategy rdf:type owl:NamedIndividual ,
                               :ContentAdaptationStrategy ;
                      rdfs:comment "Represents the absence of content adaptation strategy."@en ;
                      rdfs:label "No Adaptation Strategy"@en .


###  http://www.gsi.upm.es/ontologies/amor/experiments/ns#NoCooperationEmotionRecognition
:NoCooperationEmotionRecognition rdf:type owl:NamedIndividual ,
                                          :EmotionRecognitionCooperationStrategy ;
                                 rdfs:comment "Represents the absence of cooperation in emotion recognition in an experiment."@en ;
                                 rdfs:label "No Cooperation Emotion Recognition"@en .


###  http://www.gsi.upm.es/ontologies/amor/experiments/ns#NoCooperationRobot
:NoCooperationRobot rdf:type owl:NamedIndividual ,
                             :RobotCooperationStrategy ;
                    rdfs:comment "Represents the absence of cooperation in robot in an experiment."@en ;
                    rdfs:label "No Cooperation Robot"@en .


###  http://www.gsi.upm.es/ontologies/amor/experiments/ns#NoExpresivity
:NoExpresivity rdf:type owl:NamedIndividual ,
                        :ExpresivityCategory ;
               rdfs:comment "Represents the absence of expresivity in a character."@en ;
               rdfs:label "No Expresivity"@en .


###  http://www.gsi.upm.es/ontologies/amor/experiments/ns#NoSemanticCooperation
:NoSemanticCooperation rdf:type owl:NamedIndividual ,
                                :SemanticCooperationStrategy ;
                       rdfs:comment "Represents the absence of semantic cooperation in an experiment."@en ;
                       rdfs:label "No Semantic Cooperation"@en .


###  http://www.gsi.upm.es/ontologies/amor/experiments/ns#SentimentDisimilarity
:SentimentDisimilarity rdf:type owl:NamedIndividual ,
                                :RecommendationCriterion ;
                       rdfs:comment "Recommends elements with an opposite sentiment value"@en ;
                       rdfs:label "Opposite Sentiment Recommendation Strategy"@en .


###  http://www.gsi.upm.es/ontologies/amor/experiments/ns#SentimentSimilarity
:SentimentSimilarity rdf:type owl:NamedIndividual ,
                              :RecommendationCriterion ;
                     rdfs:comment "Recommends elements with a similar sentiment value"@en ;
                     rdfs:label "Similar Sentiment Recommendation Strategy"@en .


#################################################################
#    Annotations
#################################################################

:hasBackgroundScenario rdfs:comment "Relates an experiment with the background scenario used."@en ;
                       rdfs:label "has background scenario"@en .


:hasPhysicalMovement rdfs:comment "Relates an experiment with the physical movement used."@en ;
                     rdfs:label "has physical movement"@en .


:hasPreferredEntity rdfs:comment "Relates an experimentation subject with its preferred entities."@en ;
                    rdfs:label "has preferred entities"@en .


:hasRobotActor rdfs:comment "Relates a robot role with the robot actor."@en ;
               rdfs:label "has robot actor"@en .


:hasRobotRole rdfs:comment "Relates a robot cooperation strategy with the robot role."@en ;
              rdfs:label "has robot role"@en .


:usesAggregatedData rdfs:comment "Relates an experiment with the aggregated data used."@en ;
                    rdfs:label "uses aggregated data"@en .


:usesLanguage rdfs:comment "Relates a digital newspaper experiment with the language used in the experiment."@en ;
              rdfs:label "uses language"@en .


###  Generated by the OWL API (version 5.1.18) https://github.com/owlcs/owlapi/
