@prefix amor: <http://www.gsi.upm.es/ontologies/amor/ns#> .
@prefix dc: <http://purl.org/dc/terms/> .
@prefix marl: <http://www.gsi.upm.es/ontologies/marl/ns#> .
@prefix mls: <http://www.w3.org/ns/mls#> .
@prefix nif: <http://persistence.uni-leipzig.org/nlp2rdf/ontologies/nif-core#> .
@prefix oa: <http://www.w3.org/ns/oa#> .
@prefix onyx: <http://www.gsi.upm.es/ontologies/onyx/ns#> .
@prefix owl: <http://www.w3.org/2002/07/owl#> .
@prefix prov: <http://www.w3.org/ns/prov#> .
@prefix rdfs: <http://www.w3.org/2000/01/rdf-schema#> .
@prefix schema: <http://schema.org/> .
@prefix vann: <http://purl.org/vocab/vann/> .
@prefix xsd: <http://www.w3.org/2001/XMLSchema#> .

<http://www.gsi.upm.es/ontologies/amor/ns>
  a owl:Ontology ;
  rdfs:label "AMOR Moral Values Ontology"@en ;
  owl:versionInfo "1.0.0"^^xsd:string ;
  owl:versionIRI <http://www.gsi.upm.es/ontologies/amor/ns/1.0.0> ;
  dc:title "AMOR Moral Values Ontology"@en ;
  dc:creator "Sergio Muñoz López"@es ,
    "Álvaro Carrera Barroso"@es ,
    "Juan Fernando Sánchez Rada"@es;
  dc:publisher <http://www.gsi.upm.es> ;
  rdfs:comment "AMOR is an ontology designed for representing moral values analysis and annotations in textual sources."@en ;
  dc:description "AMOR is an ontology designed for representing moral values and value annotations in textual sources."@en ;
  vann:preferredNamespacePrefix "amor" ;
  vann:preferredNamespaceUri "http://www.gsi.upm.es/ontologies/amor/ns#" .

amor:AnalysedEntity
  a owl:Class ;
  rdfs:subClassOf prov:Entity ;
  rdfs:label "Analysed Entity"@en ;
  rdfs:comment "Represents any analysed entity that is used as a source of the analysis. It be text, such as a string or a news article; but it can be an agent; i.e. a human or a robot analysed using the results of a questionnarie."@en .

amor:MoralValueAnnotation
  a owl:Class ;
  rdfs:subClassOf prov:Entity, oa:Annotation ;
  rdfs:label "Moral Value Annotation"@en ;
  rdfs:comment "Represents a value annotation extracted from textual sources."@en .

amor:ClickBaitAnnotation
  a owl:Class ;
  rdfs:subClassOf prov:Entity, oa:Annotation ;
  rdfs:label "Clickbait Annotation"@en ;
  rdfs:comment "Represents a clickbait annotation extracted from textual sources."@en .

amor:EntityAnnotation
  a owl:Class ;
  rdfs:subClassOf prov:Entity, oa:Annotation ;
  rdfs:label "NER Annotation"@en ;
  rdfs:comment "Represents an entity found in textual sources."@en .

amor:SentimentAnnotation
  a owl:Class ;
  rdfs:subClassOf prov:Entity, nif:Opinion, oa:Annotation ;
  rdfs:label "sentiment annotation"@en ;
  rdfs:comment "Represents an opinion detected in textual sources."@en .

amor:EmotionAnnotation
  a owl:Class ;
  rdfs:subClassOf prov:Entity, onyx:EmotionSet, oa:Annotation ;
  rdfs:label "emotion annotation"@en ;
  rdfs:comment "Represents an emotion detected in textual sources."@en .

amor:AnnotationAnalysis
  a owl:Class ;
  rdfs:subClassOf prov:Activity ;
  rdfs:label "Annotation Analysis"@en ;
  rdfs:comment "Represents the activity of generating annotations of some type for a specific resource."@en .

amor:DiffBotAnalysis
  a owl:Class ;
  rdfs:subClassOf amor:AnnotationAnalysis ;
  rdfs:label "DiffBot Analysis"@en ;
  rdfs:comment "Represents the activity of analyzing text using DiffBot."@en .

amor:NamedEntityRecognitionAnalysis
  a owl:Class ;
  rdfs:subClassOf amor:AnnotationAnalysis ;
  rdfs:label "Named Entity Recognition Analysis"@en ;
  rdfs:comment "Represents the activity of analyzing text for named entities."@en .

amor:ClickBaitAnalysis
  a owl:Class ;
  rdfs:subClassOf amor:AnnotationAnalysis ;
  rdfs:label "Clickbait Analysis"@en ;
  rdfs:comment "Represents the activity of analyzing text for clickbait."@en .

amor:EmotionAnalysis
  a owl:Class ;
  owl:sameAs onyx:EmotionAnalysis ;
  rdfs:subClassOf amor:AnnotationAnalysis ;
  rdfs:label "Emotion Analysis"@en ;
  rdfs:comment "Represents the activity of analyzing text for emotions."@en .

amor:SentimentAnalysis
  a owl:Class ;
  owl:sameAs marl:SentimentAnalysis ;
  rdfs:subClassOf amor:AnnotationAnalysis ;
  rdfs:label "Sentiment Analysis"@en ;
  rdfs:comment "Represents the activity of analyzing text for sentiment."@en .

amor:MoralValueAnalysis
  a owl:Class ;
  rdfs:subClassOf amor:AnnotationAnalysis ;
  rdfs:label "Moral Value Analysis"@en ;
  rdfs:comment "Represents the activity of analyzing text for moral values."@en .

amor:MoralProfile
    a owl:Class ;
    rdfs:subClassOf amor:MoralValueAnalysis ;
    rdfs:label "Moral Profile"@en ;
    rdfs:comment "Represents the moral profile analysis of an agent."@en .

amor:hasMoralProfile
    a owl:ObjectProperty ;
    rdfs:domain prov:Agent ;
    rdfs:range amor:MoralProfile ;
    rdfs:label "has moral profile"@en ;
    rdfs:comment "Relates an agent (human or not) with its moral profile."@en .

amor:MoralValueModel
  a owl:Class ;
  rdfs:subClassOf prov:Entity ;
  rdfs:label "Moral Value Model"@en ;
  rdfs:comment "Represents a model for categorizing moral values."@en .

amor:MoralValueCategory
  a owl:Class ;
  rdfs:subClassOf prov:Entity ;
  rdfs:label "Moral Value Category"@en ;
  rdfs:comment "Represents a category of moral values."@en .

amor:NonMoral a amor:MoralValueCategory ;
  rdfs:label "Non Moral"@en ;
  rdfs:comment "Represents a non moral value. This indicates that the text does not contain any trace of moral values."@en .

amor:Neutral a amor:MoralValueCategory ;
  owl:sameAs amor:NonMoral ;
  rdfs:label "Neutral"@en ;
  rdfs:comment "Represents a neutral moral value. This indicates that the text does not contain any trace of moral values."@en .

amor:NonEmotion a onyx:EmotionCategory ;
  rdfs:label "Non Emotion"@en ;
  rdfs:comment "Represents a non emotion. This indicates that the text does not contain any trace of emotions."@en .

amor:NeutralEmotion a onyx:EmotionCategory ;
  owl:sameAs amor:NonEmotion ;
  rdfs:label "Neutral Emotion"@en ;
  rdfs:comment "Represents a neutral emotion. This indicates that the text does not contain any trace of emotions."@en .

amor:MLEntity
  a owl:Class ;
  rdfs:subClassOf prov:Entity ;
  rdfs:subClassOf mls:InformationEntity ;
  rdfs:label "Machine Learning Entity"@en ;
  rdfs:comment "Represents any entity related with a Machine Learning process. It is a subclass of mls:Entity and prov:Entity."@en .

amor:MLProcess
  a owl:Class ;
  rdfs:subClassOf prov:Activity ;
  rdfs:subClassOf mls:Run ;
  rdfs:label "Machine Learning Process"@en ;
  rdfs:comment "Represents a process related with Machine Learning that generates some output, such as a mls:Model or any other mls:InformationEntity."@en .

amor:headlineCategory
  a owl:ObjectProperty ;
  rdfs:label "headline category"@en ;
  rdfs:domain amor:ClickBaitAnnotation ;
  rdfs:range amor:ClickBaitHeadlineCategory ;
  rdfs:comment "Specifies the category of the clickbait headline."@en .

amor:ClickBaitHeadlineCategory
  a owl:Class ;
  rdfs:subClassOf prov:Entity ;
  rdfs:label "Clickbait Category"@en ;
  rdfs:comment "Represents a category of clickbait."@en .

amor:ClickBaitHeadline a amor:ClickBaitHeadlineCategory ;
  rdfs:label "Clickbait Headline"@en ;
  rdfs:comment "Represents a clickbait headline category. This means that it is considered clickbait."@en .

amor:DescriptiveHeadline a amor:ClickBaitHeadlineCategory ;
  rdfs:label "Descriptive Headline"@en ;
  rdfs:comment "Represents a descriptive headline category. This means that it is not considered clickbait."@en .

# Replace with itsrdf:taConfidence
#:confidence
#  a owl:DatatypeProperty ;
#  rdfs:label "confidence"@en ;
#  rdfs:domain amor:MoralValueAnnotation ;
#  rdfs:range xsd:float ;
#  rdfs:comment "The confidence score of the moral value annotation, ranging from 0 to 1."@en .
#

amor:hasMoralValueCategory
  a owl:ObjectProperty ;
  rdfs:subPropertyOf prov:hadMember ;
  rdfs:label "has moral value category"@en ;
  rdfs:domain [
    a owl:Class ;
    owl:unionOf (
     amor:MoralValueAnnotation 
     amor:MoralValueModel
   )
  ] ;
  rdfs:range amor:MoralValueCategory ;
  rdfs:comment "Specifies the category of the moral value."@en .

amor:usedMoralValueModel
  a owl:ObjectProperty ;
  rdfs:subPropertyOf prov:used ;
  rdfs:label "used moral value model"@en ;
  rdfs:domain amor:MoralValueAnalysis ;
  rdfs:range amor:MoralValueModel ;
  rdfs:comment "Specifies the moral value model used in the analysis."@en .

amor:analysed
  a owl:ObjectProperty ;
  rdfs:subPropertyOf prov:used ;
  rdfs:label "analysed"@en ;
  rdfs:domain amor:AnnotationAnalysis ;
  rdfs:range amor:AnalysedEntity ;
  rdfs:comment "This property relates the analysis activity with the resource that is analysed."@en .

# Removed in favor of oa:Annotation and oa:hasTarget
#amor:annotated
#  a owl:ObjectProperty ;
#  rdfs:subPropertyOf prov:wasDerivedFrom ;
#  rdfs:label "annotated"@en ;
#  rdfs:domain amor:MoralValueAnnotation ;
#  rdfs:range amor:AnalysedEntity ;
#  rdfs:comment "This property relates the ValueAnnotation activity with the resource that is annotated."@en .

amor:usedMLModel
  a owl:ObjectProperty ;
  rdfs:subPropertyOf prov:used ;
  rdfs:label "used machine learning model"@en ;
  rdfs:domain prov:Activity ;
  rdfs:range mls:Model ;
  rdfs:comment "This property relates an activity (such as a MoralAnalysis) with the Machine Learning Model (mls:Model) used to carry out the activity."@en .

amor:usedDataset
  a owl:ObjectProperty ;
  rdfs:subPropertyOf prov:used ;
  rdfs:label "used dataset"@en ;
  rdfs:domain prov:Activity ;
  rdfs:range [
        a owl:Class ;
        owl:unionOf (
            mls:Dataset
            schema:Dataset
        )
    ] ;
  rdfs:comment "This property relates an activity (such as a SentimentAnalysis) with the Dataset or the Corpus (mls:Dataset) used to carry out the analysis." .